hol/cake_sem/p4_cake_exec_sem_completenessScript.sml
@@ -1,0 +1,2666 @@
+open HolKernel boolLib Parse bossLib;
+
+val _ = new_theory "p4_cake_exec_sem_completeness";
+
+open p4Theory p4_auxTheory p4_cake_exec_semTheory;
+open p4_cake_transformTheory;
+
+Definition dict_bij_def:
+ dict_bij dict =
+  !k v.
+  MEM (k,v) dict ==>
+  UNIQUE k (MAP FST dict) /\ UNIQUE v (MAP SND dict)
+End
+
+Theorem UNIQUE_HEAD:
+!x xs. UNIQUE x (x::xs) <=> ~MEM x xs
+Proof
+rpt strip_tac >>
+EQ_TAC >- (
+ rpt strip_tac >>
+ gs[listTheory.UNIQUE_DEF] >>
+ Cases_on ‘L1’ >> (
+   gvs[]
+ )
+) >>
+rpt strip_tac >>
+gs[listTheory.UNIQUE_DEF] >>
+qexistsl_tac [‘[]’, ‘xs’] >>
+gs[]
+QED
+
+Theorem UNIQUE_TAIL:
+!x x' xs. (UNIQUE x (x'::xs) /\ x ≠ x') ==> UNIQUE x xs
+Proof
+rpt strip_tac >>
+gs[listTheory.UNIQUE_DEF] >>
+Cases_on ‘L1’ >> (
+ gvs[]
+) >>
+qexistsl_tac [‘t’, ‘L2’] >>
+gs[]
+QED
+
+Theorem TWO_UNIQUE_LEMMA:
+!dict v.
+UNIQUE v (MAP SND dict) ==>
+!k. MEM (k,v) dict ==> !k'. k' ≠ k ==> ~MEM (k',v) dict
+Proof
+Induct >- (
+ gvs[listTheory.MEM]
+) >>
+Cases_on ‘h’ >> rename1 ‘(key, val)::t’ >>
+rpt strip_tac >>
+gvs[UNIQUE_HEAD, listTheory.MEM, listTheory.MEM_MAP] >>
+Cases_on ‘v = val’ >- (
+ gs[listTheory.MEM_MAP, UNIQUE_HEAD]
+) >>
+metis_tac[UNIQUE_TAIL]
+QED
+
+(* TODO: Move *)
+Theorem TWO_UNIQUE:
+!k1 k2 v1 v2 dict.
+dict_bij dict ==>
+k1 <> k2 ==>
+MEM (k1,v1) dict ==>
+MEM (k2,v2) dict ==>
+v1 ≠ v2
+Proof
+rpt strip_tac >>
+gs[dict_bij_def] >>
+res_tac >>
+gvs[] >>
+metis_tac[TWO_UNIQUE_LEMMA]
+QED
+
+Theorem dict_bij_injectivity:
+!dict k1 k2 v.
+dict_bij dict ==>
+ALOOKUP dict k1 = SOME v ==>
+ALOOKUP dict k2 = SOME v ==>
+k1 = k2
+Proof
+rpt strip_tac >>
+‘MEM (k1, v) dict’ by metis_tac[alistTheory.ALOOKUP_MEM] >>
+‘MEM (k2, v) dict’ by metis_tac[alistTheory.ALOOKUP_MEM] >>
+‘UNIQUE v (MAP SND dict)’ by metis_tac[dict_bij_def] >>
+metis_tac[TWO_UNIQUE_LEMMA]
+QED
+
+(* TODO: Now the property is formulated in terms of a relation that is kept:
+
+                  exec
+              s1  ====> s2
+               |         |
+     translate |         |
+               |         |
+               v         v
+              s'1 ====> s'2
+                  exec'
+
+instead of a simulation:
+
+                  exec
+              s1  ====> s2
+               |         ^
+     translate |         | translate'
+               |         |
+               v         |
+              s'1 ====> s'2
+                  exec'
+
+*)
+
+(* TODO: Generalise from just V1Model *)
+Definition transform_ectx_def:
+ transform_ectx dict (ext_map, func_map, b_func_map) =
+  transform_ext_map dict ext_map >>=
+  \ext_map'. transform_func_map dict func_map >>=
+  \func_map'. transform_func_map dict b_func_map >>=
+  \b_func_map'. SOME (ext_map':v1model_ascope' ext_map', func_map':func_map', b_func_map':b_func_map')
+End
+
+Definition transform_frame_def:
+ transform_frame dict (funn, stmt_stack, scope_list) =
+  transform_funn dict funn >>=
+  \funn'. oFOLDR (transform_stmt dict) stmt_stack >>=
+  \stmt_stack'. transform_scope_list dict scope_list >>=
+  \scope_list'. SOME (funn':funn', stmt_stack':stmt' list, scope_list':scope_list')
+End
+
+Definition transform_frame_list_def:
+ transform_frame_list dict frame_list =
+  oFOLDR (transform_frame dict) frame_list
+End
+
+(* TODO: Generalise from V1Model *)
+Definition e_exec'_complete_def:
+ e_exec'_complete e'1 =
+  !e1 dict ext_map func_map b_func_map g_scope_list' g_scope_list scope_list' scope_list e_ctx.
+  dict_bij dict ==>
+  transform_ectx dict (ext_map, func_map, b_func_map) = SOME e_ctx ==>
+  transform_scope_list dict g_scope_list = SOME g_scope_list' ==>
+  transform_scope_list dict scope_list = SOME scope_list' ==>
+  transform_e dict e1 = SOME e'1 ==>
+  !apply_table_f pars_map tbl_map e2 e'2 frame_list frame_list'.
+  e_exec uninit_zero (apply_table_f,ext_map,func_map,b_func_map,pars_map,tbl_map) (g_scope_list:g_scope_list) (scope_list:scope_list) e1 = SOME (e2, frame_list) ==>
+  transform_e dict e2 = SOME e'2 ==>
+  transform_frame_list dict frame_list = SOME frame_list' ==>
+  e_exec' (e_ctx:v1model_ascope' e_ctx) (g_scope_list':g_scope_list') (scope_list':scope_list') e'1 = SOME (e'2, frame_list')
+End
+
+Definition w_e_exec'_complete_def:
+ (w_e_exec'_complete (w:word64, e) = e_exec'_complete e)
+End
+
+Definition l_complete_def:
+ (l_complete [] = T) /\
+ (l_complete (l:e' list) = 
+  !i e. (SOME e = oEL i l) ==> e_exec'_complete e)
+End
+(* More convenient alternate form of the above *)
+Definition l_complete_exec_def:
+ (l_complete_exec [] = T) /\
+ (l_complete_exec ((h::t):e' list) = 
+  (e_exec'_complete h /\ l_complete_exec t))
+End
+
+Definition w_e_l_exec'_complete_def:
+ (w_e_l_exec'_complete (w_e_l:(word64 # e') list) = l_complete (MAP SND w_e_l))
+End
+
+Theorem l_complete_cons:
+!h l. l_complete (h::l) ==> l_complete l
+Proof
+rpt strip_tac >>
+Induct_on ‘l’ >> (
+ gs[l_complete_def]
+) >>
+rpt strip_tac >>
+qpat_x_assum ‘!x e. _’ (fn thm => assume_tac $ Q.SPECL [‘SUC i’, ‘e’] thm) >>
+gs[] >>
+‘oEL i (h'::l) = oEL (SUC i) (h::h'::l)’ suffices_by (
+ gs[]
+) >>
+Induct_on ‘i’ >> (
+ gs[listTheory.oEL_def]
+)
+QED
+
+Theorem l_complete_equiv:
+!type l. l_complete l <=> l_complete_exec l
+Proof
+rpt strip_tac >>
+EQ_TAC >| [
+ Induct_on ‘l’ >> (
+  gs[l_complete_def, l_complete_exec_def]
+ ) >>
+ rpt strip_tac >| [
+  qpat_x_assum ‘!x e. _’ (fn thm => assume_tac $ Q.SPEC ‘0:num’ thm) >>
+  gs[listTheory.oEL_def],
+
+  ‘l_complete (h::l)’ suffices_by (
+   metis_tac[l_complete_cons]
+  ) >>
+  metis_tac[l_complete_def]
+ ],
+
+ Induct_on ‘l’ >> (
+  gs[l_complete_def, l_complete_exec_def]
+ ) >>
+ NTAC 3 strip_tac >>
+ Induct_on ‘i’ >> (
+  gs[listTheory.oEL_def]
+ ) >>
+ ‘!i e. SOME e = oEL i l ==> e_exec'_complete e’ suffices_by (
+  metis_tac[oEL_cons_PRE]
+ ) >>
+ gs[] >>
+ Cases_on ‘l’ >- (
+  gs[listTheory.oEL_def]
+ ) >>
+ metis_tac[l_complete_def]
+]
+QED
+
+Theorem l_complete_MEM:
+ !e l.
+ MEM e l ==>
+ l_complete l ==>
+ e_exec'_complete e
+Proof
+Induct_on ‘l’ >> (
+ gs[]
+) >>
+rpt strip_tac >> (
+ gs[l_complete_equiv, l_complete_exec_def]
+)
+QED
+
+Definition reverse_dict_def:
+  reverse_dict dict = MAP (\(a,b). (b,a)) dict
+End
+
+(*
+(* TODO: This should rather be "reversibility under ALOOKUP" or something *)
+Definition dict_bij_def:
+ dict_bij dict =
+  !a b.
+  ALOOKUP dict a = SOME b <=>
+  ALOOKUP (reverse_dict dict) b = SOME a
+End
+*)
+
+(* TODO: Needed? *)
+Theorem transform_v_struct_split:
+!p p' l l' dict.
+transform_v dict (v_struct (p::l)) = SOME (v'_struct (p'::l')) ==>
+transform_v dict (v_struct [p]) = SOME (v'_struct [p']) /\
+transform_v dict (v_struct l) = SOME (v'_struct l')
+Proof
+rpt strip_tac >- (
+ gs[Once transform_v_def, AllCaseEqs()] >>
+ simp[Once transform_v_def, AllCaseEqs()] >>
+ simp[Once transform_v_def, AllCaseEqs()]
+) >>
+gs[Once transform_v_def, AllCaseEqs()]
+QED
+
+Theorem lookup_transform_v_struct:
+!dict x w t t' v' v.
+ dict_bij dict ==>
+ transform_v dict (v_struct t) = SOME (v'_struct t') ==>
+ ALOOKUP t x = SOME v ==>
+ transform_v dict v = SOME v' ==>
+ ALOOKUP dict x = SOME w ==>
+ ALOOKUP t' w = SOME v'
+Proof
+rpt strip_tac >>
+(* When transforming a struct, the names of fields are translated according to dict.
+ * If an entry exists in the original table, the dictionary-translated entry must exist
+ * in the translated struct - in fact, at the same location. The value is then the translated version
+  * of the original entry. *)
+cheat
+QED
+        
+Theorem INDEX_FIND_index:
+ !a l P b.
+ INDEX_FIND 0 P l = SOME (a,b) ==>
+ INDEX_FIND 1 P l = SOME (a+1,b)
+Proof
+rpt strip_tac >>
+simp[Once listTheory.INDEX_FIND_add]
+QED
+
+(* TODO: Move? *)
+Theorem alookup_find:
+!l k v.
+(FIND (λ(k',v'). k' = k) l = SOME (k,v)) <=>
+ALOOKUP l k = SOME v
+Proof
+Induct >- (
+ gs[listTheory.FIND_def, listTheory.INDEX_FIND_def]
+) >>
+rpt strip_tac >>
+Cases_on ‘h’ >>
+gs[listTheory.FIND_def, listTheory.INDEX_FIND_def, AllCaseEqs()] >>
+Cases_on ‘q = k’ >> (
+ gs[]
+) >- (
+ (* Why metis needed here? *)
+ metis_tac[]
+) >>
+qpat_x_assum ‘!k v. _’ (fn thm => ASSUME_TAC $ Q.SPECL [‘k’, ‘v’] thm) >>
+eq_tac >- (
+ rpt strip_tac >>
+ ‘?i. INDEX_FIND 0 (λ(k',v'). k' = k) l = SOME (i, (k,v))’ suffices_by (strip_tac >> gs[]) >>
+ Cases_on ‘z’ >>
+ qexists_tac ‘q' - 1’ >>
+ gvs[] >>
+ qpat_x_assum ‘(?z. INDEX_FIND 0 (λ(k',v'). k' = k) l = SOME z ∧ (k,v) = SND z) ⇔
+        ALOOKUP l k = SOME v’ (fn thm => ALL_TAC) >>
+ gs[Once listTheory.INDEX_FIND_add] >>
+ Cases_on ‘z’ >>
+ gs[]
+) >>
+rpt strip_tac >>
+gvs[] >>
+Cases_on ‘z’ >>
+qexists_tac ‘(q' + 1, r)’ >>
+gvs[INDEX_FIND_index]
+QED
+
+(* Completeness of acc, non-recursive case *)
+Theorem e_exec'_acc_complete:
+!dict e'1 e' x c e2 e'2.
+ dict_bij dict ==>
+ is_v' e'1 ==>
+ transform_e dict e' = SOME e'1 ==>
+ ALOOKUP dict x = SOME c ==>
+ e_exec_acc (e_acc e' x) = SOME e2 ==>
+ transform_e dict e2 = SOME e'2 ==>
+ e_exec_acc' (e'_acc e'1 c) = SOME e'2
+Proof
+rpt strip_tac >>
+Cases_on ‘e'’ >> (gs[p4_exec_semTheory.e_exec_acc_def]) >>
+Cases_on ‘v’ >> (gvs[p4_exec_semTheory.e_exec_acc_def, p4_exec_semTheory.is_v_def, AllCaseEqs()]) >> (
+ gvs[transform_e_def, AllCaseEqs()] >>
+ qpat_x_assum ‘transform_v dict _ = SOME v'’ (fn thm => ASSUME_TAC $ ONCE_REWRITE_RULE [transform_v_def] thm >> gvs[listTheory.FIND_thm, e_exec_acc'_def, AllCaseEqs()]) >>
+ DISJ2_TAC >>
+ CONJ_TAC >- (
+  ‘MEM (x,c) dict’ by gs[alistTheory.ALOOKUP_MEM] >>
+  ‘MEM (x',w) dict’ by gs[alistTheory.ALOOKUP_MEM] >>
+  ‘UNIQUE c (MAP SND dict)’ by metis_tac[dict_bij_def] >>
+  ‘UNIQUE w (MAP SND dict)’ by metis_tac[dict_bij_def] >>
+  metis_tac[TWO_UNIQUE]
+ ) >>
+ (* Reversibility of v transformation *)
+ ‘ALOOKUP t x = SOME v’ by (
+  gs[GSYM alookup_find] >>
+  qpat_x_assum ‘FIND (\(k,v). k = x) t = SOME (f,v)’ (fn thm => ASSUME_TAC $ REWRITE_RULE [listTheory.FIND_def] thm) >>
+  gs[] >>
+  Cases_on ‘z’ >>
+  imp_res_tac index_find_first >>
+  gs[] >>
+  Cases_on ‘r’ >>
+  gs[]
+ ) >>
+ metis_tac[lookup_transform_v_struct]
+)
+QED
+
+Theorem unop_exec'_subtypes:
+  !uop v v'.
+  unop_exec' uop v = SOME v' ==>
+  ?b. v' = v'_bool b \/ ?bitv. v' = v'_bit bitv
+Proof
+rpt strip_tac >>
+Cases_on ‘v’ >> Cases_on ‘uop’ >> (
+ gs[unop_exec'_def]
+) >- (
+ metis_tac[]
+) >- (
+ Cases_on ‘p’ >>
+ gs[unop_exec'_def] >>
+ metis_tac[]
+) >- (
+ Cases_on ‘p’ >>
+ gs[unop_exec'_def, AllCaseEqs()] >>
+ metis_tac[]
+) >>
+metis_tac[]
+QED
+
+Theorem exec_cast'_subtypes:
+  !uop e' v' c.
+  e_exec_cast' c e' = SOME v' ==>
+  ?b. v' = v'_bool b \/ ?bitv. v' = v'_bit bitv
+Proof
+rpt strip_tac >>
+Cases_on ‘c’ >> Cases_on ‘e'’ >> (
+ gs[e_exec_cast'_def]
+) >- (
+ Cases_on ‘v’ >> (
+  gs[cast_exec_def]
+ ) >>
+ metis_tac[]
+) >>
+Cases_on ‘v’ >> (
+ gs[cast_exec_def]
+) >>
+Cases_on ‘p’ >> (
+ gs[to_bool_cast_exec_def, AllCaseEqs()]
+) >>
+metis_tac[]
+QED
+
+Theorem transform_v_struct:
+ !v' x_v_l dict.
+ transform_v dict (v_struct x_v_l) = SOME v' ==>
+ ?w_v'_l. v' = (v'_struct w_v'_l)
+Proof
+Induct >> (
+ rpt strip_tac >>
+ gs[Once transform_v_def, AllCaseEqs()]
+)
+QED
+
+Theorem transform_e_header:
+!e' x_e_l dict b.
+transform_e dict (e_header b x_e_l) = SOME e' ==>
+?w_e'_l b'. e' = e'_header b' w_e'_l
+Proof
+Induct >> (
+ rpt strip_tac >>
+ gs[Once transform_e_def, AllCaseEqs()]
+) >> (
+ qpat_x_assum ‘transform_e dict (e_header _ _) = SOME _’ (fn thm => assume_tac $ ONCE_REWRITE_RULE [transform_e_def] thm >> gvs[AllCaseEqs()])
+)
+QED
+
+Theorem transform_e_header_validity:
+!x_e_l w_e'_l dict b b'.
+transform_e dict (e_header b x_e_l) = SOME $ e'_header b' w_e'_l ==>
+b = b'
+Proof
+Induct >> Induct >> (
+ rpt strip_tac >>
+ gs[Once transform_e_def, AllCaseEqs()]
+) >- (
+ gs[Once transform_e_def, AllCaseEqs()]
+) >>
+qpat_x_assum ‘!w_e'_l'. _’ (fn thm => irule thm) >>
+qexistsl_tac [‘dict’] >>
+Cases_on ‘x_e_l’ >- (
+ gs[Once transform_e_def, AllCaseEqs()] >>
+ qpat_x_assum ‘transform_e dict (e_header b []) = SOME (e'_header b' t')’ (fn thm => assume_tac $ ONCE_REWRITE_RULE [transform_e_def] thm >> gvs[AllCaseEqs()])
+) >>
+gs[] >>
+Cases_on ‘h’ >>
+gvs[] >>
+qpat_x_assum ‘transform_e dict (e_header b _) = SOME _’ (fn thm => assume_tac $ ONCE_REWRITE_RULE [transform_e_def] thm >> gvs[AllCaseEqs()]) >>
+qpat_x_assum ‘transform_e dict (e_header b _) = SOME _’ (fn thm => assume_tac $ ONCE_REWRITE_RULE [transform_e_def] thm >> gvs[AllCaseEqs()])
+QED
+
+Theorem transform_e_subtypes:
+(!dict v e'. transform_e dict (e_v v) = SOME e' ==> ?v'. e' = e'_v v') /\
+(!dict varn e'. transform_e dict (e_var varn) = SOME e' ==> ?varn'. e' = e'_var varn') /\
+(!dict l e'. transform_e dict (e_list l) = SOME e' ==> ?l'. e' = e'_list l') /\
+(!dict e x e'. transform_e dict (e_acc e x) = SOME e' ==> ?e'' w. e' = e'_acc e'' w) /\
+(!dict u e e'. transform_e dict (e_unop u e) = SOME e' ==> ?e''. e' = e'_unop u e'') /\
+(!dict c e e'. transform_e dict (e_cast c e) = SOME e' ==> ?e''. e' = e'_cast c e'') /\
+(!dict e1 b e2 e'. transform_e dict (e_binop e1 b e2) = SOME e' ==> ?e1' e2'. e' = e'_binop e1' b e2') /\
+(!dict e1 e2 e'. transform_e dict (e_concat e1 e2) = SOME e' ==> ?e1' e2'. e' = e'_concat e1' e2') /\
+(!dict e1 e2 e3 e'. transform_e dict (e_slice e1 e2 e3) = SOME e' ==> ?e1' e2' e3'. e' = e'_slice e1' e2' e3') /\
+(!dict funn l e'. transform_e dict (e_call funn l) = SOME e' ==> ?funn' l'. e' = e'_call funn' l') /\
+(!dict e s_l_x_l x e'. transform_e dict (e_select e s_l_x_l x) = SOME e' ==> ?e'' s'_l_w_l w n_l_l. e' = e'_select e'' s'_l_w_l w n_l_l) /\
+(!dict x_e_l e'. transform_e dict (e_struct x_e_l) = SOME e' ==> ?w_e'_l. e' = e'_struct w_e'_l) /\
+(!dict b x_e_l e'. transform_e dict (e_header b x_e_l) = SOME e' ==> ?w_e'_l. e' = e'_header b w_e'_l)
+Proof
+rpt strip_tac >- (
+ gs[transform_e_def] >>
+ metis_tac[]
+) >- (
+ gs[transform_e_def] >>
+ metis_tac[]
+) >- (
+ (* List *)
+ Cases_on ‘l’ >- (
+  gs[Once transform_e_def] >>
+  metis_tac[]
+ ) >>
+ gs[Once transform_e_def, AllCaseEqs()] >>
+ metis_tac[]
+) >- (
+ gs[Once transform_e_def] >>
+ metis_tac[]
+) >- (
+ gs[Once transform_e_def] >>
+ metis_tac[]
+) >- (
+ gs[Once transform_e_def] >>
+ metis_tac[]
+) >- (
+ gs[Once transform_e_def] >>
+ metis_tac[]
+) >- (
+ gs[Once transform_e_def] >>
+ metis_tac[]
+) >- (
+ gs[Once transform_e_def] >>
+ metis_tac[]
+) >- (
+ (* Call *)
+ Cases_on ‘l’ >- (
+  gs[Once transform_e_def] >>
+  metis_tac[]
+ ) >>
+ gs[Once transform_e_def, AllCaseEqs()] >>
+ metis_tac[]
+) >- (
+ (* Select *)
+ gs[Once transform_e_def, listTheory.UNZIP_MAP] >>
+ metis_tac[]
+) >- (
+ (* Struct *)
+ Cases_on ‘x_e_l’ >- (
+  gs[Once transform_e_def] >>
+  metis_tac[]
+ ) >>
+ gs[Once transform_e_def, AllCaseEqs()] >>
+ gs[] >>
+ metis_tac[]
+) >>
+(* Header *)
+imp_res_tac transform_e_header >>
+rw[] >>
+metis_tac[transform_e_header_validity]
+QED
+
+Theorem transform_e_is_v:
+!dict e e'.
+is_v e ==>
+transform_e dict e = SOME e' ==>
+is_v' e'
+Proof
+rpt strip_tac >>
+Cases_on ‘e’ >> (
+ gs[Once transform_e_def, AllCaseEqs()] >>
+ Cases_on ‘e'’ >> ( gs[p4_exec_semTheory.is_v_def, is_v'_def] )
+)
+QED
+
+Theorem transform_e_not_is_v:
+!dict e e'.
+~is_v e ==>
+transform_e dict e = SOME e' ==>
+~is_v' e'
+Proof
+rpt strip_tac >>
+Cases_on ‘e’ >> (
+ gs[Once transform_e_def, AllCaseEqs()] >>
+ Cases_on ‘e'’ >> ( gs[p4_exec_semTheory.is_v_def, is_v'_def] )
+) >>
+gs[listTheory.UNZIP_MAP]
+QED
+
+Theorem transform_e_is_v_bit:
+!dict e e'.
+is_v_bit e ==>
+transform_e dict e = SOME e' ==>
+is_v_bit' e'
+Proof
+rpt strip_tac >>
+Cases_on ‘e’ >> (
+ gs[Once transform_e_def, Once transform_v_def, AllCaseEqs()] >>
+ Cases_on ‘e'’ >> ( gvs[p4_exec_semTheory.is_v_bit_def, is_v_bit'_def] ) >>
+ Cases_on ‘v’ >> Cases_on ‘v'’ >> ( gs[p4_exec_semTheory.is_v_bit_def, is_v_bit'_def] )
+)
+QED
+
+Theorem transform_e_not_is_v_bit:
+!dict e e'.
+~is_v_bit e ==>
+transform_e dict e = SOME e' ==>
+~is_v_bit' e'
+Proof
+rpt strip_tac >>
+gs[] >>
+Cases_on ‘e’ >> (gs[p4_exec_semTheory.is_v_bit_def]) >- (
+ Cases_on ‘v’ >> (gs[p4_exec_semTheory.is_v_bit_def]) >> (
+  gvs[Once transform_e_def, AllCaseEqs()] >>
+  Cases_on ‘v'’ >> (
+   gs[is_v_bit'_def, Once transform_v_def, AllCaseEqs()]
+  )
+ )
+) >> (
+ gvs[Once transform_e_def, AllCaseEqs()] >>
+ gs[is_v_bit'_def]
+) >>
+gvs[listTheory.UNZIP_MAP, is_v_bit'_def]
+QED
+
+(* Reverse implication *)
+Theorem transform_scope_list_lookup:
+!dict g_scope_list scope_list g_scope_list' scope_list' varn varn' v v'.
+dict_bij dict ==>
+transform_scope_list dict g_scope_list = SOME g_scope_list' ==>
+transform_scope_list dict scope_list = SOME scope_list' ==>
+transform_varn dict varn = SOME varn' ==>
+lookup_vexp2 scope_list g_scope_list varn = SOME v ==>
+transform_v dict v = SOME v' ==> 
+lookup_vexp2' scope_list' g_scope_list' varn' = SOME v'
+Proof
+(* Looking up a variable in scopes will return the translated value of the
+ * result of looking up the translated variable name. *)
+rpt strip_tac >>
+gvs[lookup_vexp2_def, lookup_vexp2'_def, lookup_map_def, lookup_map'_def, topmost_map_def, AllCaseEqs()] >>
+(* TODO: Formulate separate theorem here, that states the correspondence between the scopes and index returned *)
+cheat
+QED
+
+Theorem unred_mem_index_same:
+unred_mem_index' [] = NONE <=>
+unred_mem_index [] = NONE
+Proof
+gs[unred_mem_index_def, unred_mem_index'_def, unred_mem_def, unred_mem'_def, AllCaseEqs(), listTheory.INDEX_FIND_def]
+QED
+
+Theorem e_exec'_completeness_var:
+!v.
+e_exec'_complete (e'_var v)
+Proof
+gs[e_exec'_complete_def] >>
+rpt strip_tac >>
+(* 1. Rewrite transformation of initial state *)
+qpat_x_assum ‘transform_e dict e1 = SOME (e'_var v)’ (fn thm => ASSUME_TAC $ ONCE_REWRITE_RULE [transform_e_def] thm >> gvs[listTheory.UNZIP_MAP, AllCaseEqs()]) >>
+(* 2. Rewrite execution *)
+gvs[e_exec'_def, p4_exec_semTheory.e_exec_def, AllCaseEqs()] >>
+(* 3. Rewrite transformation of final state *)
+gvs[transform_e_def, transform_frame_list_def, oFOLDR_def] >>
+metis_tac[transform_scope_list_lookup]
+QED
+
+Theorem e_exec'_completeness_acc:
+!e c.
+e_exec'_complete e ==>
+e_exec'_complete (e'_acc e c)
+Proof
+gs[e_exec'_complete_def] >>
+rpt strip_tac >>
+(* 1. Rewrite transformation of initial state *)
+qpat_x_assum ‘transform_e dict e1 = SOME (e'_acc e c)’ (fn thm => ASSUME_TAC $ ONCE_REWRITE_RULE [transform_e_def] thm >> gvs[listTheory.UNZIP_MAP, AllCaseEqs()]) >>
+(* 2. Rewrite execution *)
+gvs[e_exec'_def, p4_exec_semTheory.e_exec_def, AllCaseEqs()] >> (
+ gvs[transform_frame_list_def, oFOLDR_def]
+) >- (
+ (* Case 2a: e' is value *)
+ ‘is_v' e’ by metis_tac[transform_e_is_v] >> gs[] >>
+ metis_tac[e_exec'_acc_complete]
+) >>
+(* Case 2b: e' is not value *)
+‘~is_v' e’ by metis_tac[transform_e_not_is_v] >> gs[] >>
+(* 3. Rewrite transformation of final state *)
+qpat_x_assum ‘transform_e dict (e_acc e_v_struct' x) = SOME e'2’ (fn thm => ASSUME_TAC $ ONCE_REWRITE_RULE [transform_e_def] thm >> gvs[app_opt_def, AllCaseEqs()]) >>
+(* 4. Use induction hypothesis *)
+metis_tac[]
+QED
+
+Theorem e_exec'_completeness_unop:
+!e u.
+e_exec'_complete e ==>
+e_exec'_complete (e'_unop u e)
+Proof
+gs[e_exec'_complete_def] >>
+rpt strip_tac >>
+(* 1. Rewrite transformation of initial state *)
+qpat_x_assum ‘transform_e dict e1 = SOME (e'_unop u e)’ (fn thm => ASSUME_TAC $ ONCE_REWRITE_RULE [transform_e_def] thm >> gvs[listTheory.UNZIP_MAP, AllCaseEqs()]) >>
+(* 2. Rewrite execution *)
+gvs[e_exec'_def, p4_exec_semTheory.e_exec_def, AllCaseEqs()] >> (
+ gvs[transform_frame_list_def, oFOLDR_def]
+) >- (
+ (* Case 2a: e' is value *)
+ ‘is_v' e’ by metis_tac[transform_e_is_v] >> gs[] >>
+(* TODO: Make separate lemma from the below... *)
+ qpat_x_assum ‘!e1. _’ (fn thm => ALL_TAC) >>
+ gvs[Once transform_e_def] >>
+ (* Obtain the e_v subtypes *)
+ Cases_on ‘e'’ >> (
+  gs[p4_exec_semTheory.is_v_def]
+ ) >>
+ Cases_on ‘e’ >> (
+  gs[is_v'_def]
+ ) >> 
+ Cases_on ‘u’ >> (
+  gs[e_exec_unop'_def, p4_exec_semTheory.e_exec_unop_def]
+ ) >> (
+  Cases_on ‘v''’ >> Cases_on ‘v'''’ >>
+  gs[Once transform_e_def] >>
+  rfs[Once transform_v_def] >>
+  gvs[unop_exec'_def, p4_exec_semTheory.e_exec_unop_def, p4_exec_semTheory.unop_exec_def] >>
+  gvs[AllCaseEqs()] >>
+  Cases_on ‘p’ >> (
+   gs[unop_exec'_def, bitv_1comp_def, bitv_bl_unop_def, bitstringTheory.bnot_def] >>
+   gs[bitv_2comp_def, AllCaseEqs()] >>
+   (* TODO: Issues for "bitv_unop unop_neg_signed" since this is only defined for up to
+    * a certain bitwidth... :(
+    *
+    * Solutions: Either make the CakeML-exportable semantics return NONE for widths over
+    * 128 at an earlier stage, or have a fallback solution in the regular semantics for
+    * widths over 128 *)
+   cheat
+  )
+ )
+) >>
+(* Case 2b: e' is not value *)
+‘~is_v' e’ by metis_tac[transform_e_not_is_v] >> gs[] >>
+(* 3. Rewrite transformation of final state *)
+qpat_x_assum ‘transform_e dict (e_unop u e'') = SOME e'2’ (fn thm => ASSUME_TAC $ ONCE_REWRITE_RULE [transform_e_def] thm >> gvs[app_opt_def, AllCaseEqs()]) >>
+(* 4. Use induction hypothesis *)
+metis_tac[]
+QED
+
+Theorem e_exec'_completeness_cast:
+!e c.
+e_exec'_complete e ==>
+e_exec'_complete (e'_cast c e)
+Proof
+gs[e_exec'_complete_def] >>
+rpt strip_tac >>
+(* 1. Rewrite transformation of initial state *)
+qpat_x_assum ‘transform_e dict e1 = SOME (e'_cast c e)’ (fn thm => ASSUME_TAC $ ONCE_REWRITE_RULE [transform_e_def] thm >> gvs[listTheory.UNZIP_MAP, AllCaseEqs()]) >>
+(* 2. Rewrite execution *)
+gvs[e_exec'_def, p4_exec_semTheory.e_exec_def, AllCaseEqs()] >> (
+ gvs[transform_frame_list_def, oFOLDR_def]
+) >- (
+ (* Case 2a: e' is value *)
+ ‘is_v' e’ by metis_tac[transform_e_is_v] >> gs[] >>
+(* TODO: Make separate lemma from the below... *)
+ qpat_x_assum ‘!e1. _’ (fn thm => ALL_TAC) >>
+ gvs[Once transform_e_def] >>
+ Cases_on ‘e''’ >> (
+  gs[p4_exec_semTheory.is_v_def]
+ ) >>
+ Cases_on ‘e’ >> (
+  gs[is_v'_def]
+ ) >> 
+ Cases_on ‘c’ >> (
+  gs[e_exec_cast'_def, p4_exec_semTheory.e_exec_cast_def]
+ ) >> (
+  Cases_on ‘v''’ >> Cases_on ‘v'''’ >>
+  gs[Once transform_e_def] >>
+  rfs[Once transform_v_def] >>
+  gvs[cast_exec_def, p4_exec_semTheory.e_exec_cast_def, p4_exec_semTheory.cast_exec_def, to_bool_cast_exec_def, p4_exec_semTheory.to_bool_cast_exec_def] >>
+  gvs[AllCaseEqs()]
+ )
+) >>
+(* Case 2b: e' is not value *)
+‘~is_v' e’ by metis_tac[transform_e_not_is_v] >> gs[] >>
+(* 3. Rewrite transformation of final state *)
+qpat_x_assum ‘transform_e dict (e_cast c e') = SOME e'2’ (fn thm => ASSUME_TAC $ ONCE_REWRITE_RULE [transform_e_def] thm >> gvs[app_opt_def, AllCaseEqs()]) >>
+(* 4. Use induction hypothesis *)
+metis_tac[]
+QED
+
+(* If you transform a struct used for matching in select,
+ * and if you transform the s_list_x_list used for matching,
+ * then a NONE result in matching is preserved. *)
+Theorem transform_select_NONE:
+transform_e dict (e_v (v_struct x_v_l)) =
+ SOME (e'_v (v'_struct w_v'_l)) ==>
+FIND (\(s_list,x'). match_all (ZIP (SND (UNZIP x_v_l),s_list)))
+ s_list_x_list = NONE ==>
+oFOLDR (oFOLDR (transform_s dict)) (MAP FST s_list_x_list) =
+ SOME s_n_list_list' ==>
+oFOLDR (ALOOKUP dict) (MAP SND s_list_x_list) = SOME x_list' ==>
+match_all_first (SND (UNZIP w_v'_l))
+ (ZIP (MAP FST (MAP UNZIP s_n_list_list'),x_list')) = NONE
+Proof
+cheat
+QED
+
+Theorem transform_select_SOME:
+transform_v dict (v_struct x_v_l) =
+ SOME (v'_struct w_v'_l) ==>
+FIND (\(s_list,x'). match_all (ZIP (SND (UNZIP x_v_l),s_list)))
+ s_list_x_list = SOME (s_list,x'') ==>
+oFOLDR (oFOLDR (transform_s dict)) (MAP FST s_list_x_list) =
+ SOME s_n_list_list' ==>
+oFOLDR (ALOOKUP dict) (MAP SND s_list_x_list) = SOME x_list' ==>
+match_all_first (SND (UNZIP w_v'_l))
+ (ZIP (MAP FST (MAP UNZIP s_n_list_list'),x_list')) = SOME word'
+Proof
+cheat
+QED
+
+Theorem e_exec'_completeness_select:
+!e l0 c l.
+e_exec'_complete e ==>
+e_exec'_complete (e'_select e l0 c l)
+Proof
+gs[e_exec'_complete_def] >>
+rpt strip_tac >>
+(* 1. Rewrite transformation of initial state *)
+qpat_x_assum ‘transform_e dict e1 = SOME (e'_select e l0 c l)’ (fn thm => ASSUME_TAC $ ONCE_REWRITE_RULE [transform_e_def] thm >> gvs[listTheory.UNZIP_MAP, AllCaseEqs()]) >>
+(* 2. Rewrite execution *)
+gvs[e_exec'_def, p4_exec_semTheory.e_exec_def, AllCaseEqs()] >> (
+ gvs[transform_frame_list_def, oFOLDR_def]
+) >- (
+ (* Case 2a: e''' is a value *)
+ qpat_x_assum ‘!e1. _’ (fn thm => ALL_TAC) >>
+ ‘is_v' e’ by metis_tac[transform_e_is_v] >> gs[] >>
+ (* First, get result of operation on cake_sem in proof goal *)
+ Cases_on ‘e’ >> (gs[is_v'_def]) >>
+ simp[e_exec_select'_def, AllCaseEqs()] >>
+ gs[] >>
+ (* Then, obtain everything involved
+  * in the operation from regular semantics by case analysis *)
+ Cases_on ‘e'''’ >> (gs[p4_exec_semTheory.is_v_def]) >>
+ (* Apply regular operation *)
+ gvs[p4_exec_semTheory.e_exec_select_def, AllCaseEqs()] >- (
+  (* Connect the concrete values via translation *)
+  qexists_tac ‘c’ >>
+  gvs[transform_e_def, transform_v_def]
+ ) >- (
+  qexists_tac ‘c’ >>
+  gvs[transform_e_def, transform_v_def]
+ ) >- ( 
+  qexists_tac ‘c’ >>
+  gvs[transform_e_def, transform_v_def]
+ ) >- (
+  (* Struct: case no match *)
+  qexists_tac ‘c’ >>
+  CONJ_TAC >- (
+   NTAC 3 DISJ2_TAC >> DISJ1_TAC >>
+   (* TODO: Result of transforming v_struct is a v'_struct *)
+   ‘?w_v'_l. v = v'_struct w_v'_l’ by (gs[transform_e_def] >> metis_tac[transform_v_struct]) >>
+   gvs[] >>
+   DISJ1_TAC >>
+   (* Property of how the s_list_x_list is transformed -
+    * the result of no matches must be preserved *)
+   metis_tac[transform_select_NONE]
+  ) >>
+  gvs[Once transform_e_def, transform_v_def]
+ ) >- (
+  (* Struct: case SOME match *)
+  qpat_x_assum ‘transform_e dict (e_v (v_str x'')) = SOME e'2’ (fn thm => assume_tac $ ONCE_REWRITE_RULE [transform_e_def] thm >> gvs[AllCaseEqs()]) >>
+  gs[transform_v_def] >>
+  qexists_tac ‘word'’ >>
+  CONJ_TAC >- (
+   NTAC 3 DISJ2_TAC >> DISJ1_TAC >>
+   (* Property of how the s_list_x_list is transformed -
+    * the result of matches must be preserved *)
+   qpat_x_assum ‘transform_e dict (e_v (v_struct x_v_l)) = SOME (e'_v v)’ (fn thm => assume_tac $ ONCE_REWRITE_RULE [transform_e_def] thm >> gvs[AllCaseEqs()]) >>
+   ‘?w_v'_l. v = v'_struct w_v'_l’ by metis_tac[transform_v_struct] >>
+   gvs[] >>
+   DISJ2_TAC >>
+   metis_tac[transform_select_SOME]
+  ) >>
+  gvs[]
+ ) >- (
+  (* Header *)
+  qexists_tac ‘c’ >>
+  gvs[Once transform_e_def, transform_v_def] >>
+  gvs[transform_e_def, Once transform_v_def, AllCaseEqs()]
+ ) >> (
+  gvs[transform_e_def, transform_v_def]
+ )
+) >>
+(* Case 2b: e2' is not value *)
+‘~is_v' e’ by metis_tac[transform_e_not_is_v] >> gs[] >>
+(* 3. Rewrite transformation of final state *)
+qpat_x_assum ‘transform_e dict (e_select e' s_list_x_list x') = SOME e'2’ (fn thm => ASSUME_TAC $ ONCE_REWRITE_RULE [transform_e_def] thm >> gvs[listTheory.UNZIP_MAP, AllCaseEqs()]) >>
+(* 4. Use induction hypothesis *)
+metis_tac[]
+QED
+
+Theorem transform_list_LENGTH:
+!t t' dict.
+transform_e dict (e_list t) = SOME (e'_list t') ==>
+LENGTH t = LENGTH t'
+Proof
+Induct >> (
+ rpt strip_tac >>
+ gs[Once transform_e_def, AllCaseEqs()]
+) >>
+qpat_x_assum ‘transform_e dict (e_list _) = SOME _’ (fn thm => assume_tac $ ONCE_REWRITE_RULE [transform_e_def] thm >> gvs[AllCaseEqs()]) >>
+qpat_x_assum ‘!t'' dict'. _’ (fn thm => irule thm) >>
+qexists_tac ‘dict’ >>
+Cases_on ‘t’ >> Cases_on ‘t''’ >> (
+ gs[]
+) >> (
+qpat_x_assum ‘transform_e dict (e_list _) = SOME _’ (fn thm => assume_tac $ ONCE_REWRITE_RULE [transform_e_def] thm >> gvs[AllCaseEqs()])
+)
+QED
+
+Theorem transform_list_MEM:
+!t t' e' dict.
+transform_e dict (e_list t) = SOME (e'_list t') ==>
+MEM e' t' ==>
+?e. transform_e dict e = SOME e'
+Proof
+Induct_on ‘t’ >- (
+ gs[transform_e_def]
+) >>
+rpt strip_tac >>
+qpat_x_assum ‘transform_e dict (e_list (h::t)) = SOME (e'_list t')’
+ (fn thm => assume_tac $ ONCE_REWRITE_RULE [transform_e_def] thm >> 
+  gvs[AllCaseEqs()]) >>
+metis_tac[]
+QED
+
+(* TODO: Requires injectivity of transform_e? *)
+Theorem transform_list_EL:
+!l l' ei ei' i dict.
+transform_e dict (e_list l) = SOME (e'_list l') ==>
+oEL i l' = SOME ei' ==>
+oEL i l = SOME ei ==>
+transform_e dict ei = SOME ei'
+Proof
+Induct_on ‘l’ >- (
+ rpt strip_tac >>
+ gvs[Once transform_e_def, listTheory.oEL_def]
+) >>
+rpt strip_tac >>
+qpat_x_assum ‘transform_e dict (e_list (h::l)) = SOME (e'_list l')’
+ (fn thm => assume_tac $ ONCE_REWRITE_RULE [transform_e_def] thm >> 
+  gvs[AllCaseEqs()]) >>
+Cases_on ‘i’ >> (
+ gvs[listTheory.oEL_def]
+) >>
+gs[listTheory.oEL_EQ_EL]
+QED
+
+Theorem l_complete_mem:
+!l e.
+l_complete l ==>
+MEM e l ==>
+e_exec'_complete e
+Proof
+Cases_on ‘l’ >> (
+ gs[l_complete_def]
+) >>
+rpt strip_tac >- (
+ gvs[] >>
+ qpat_x_assum ‘!i e. _’ (fn thm => irule thm) >>
+ qexists_tac ‘0’ >>
+ gs[listTheory.oEL_def]
+) >>
+qpat_x_assum ‘!i e. _’ (fn thm => irule thm) >>
+gs[listTheory.MEM_EL] >>
+qexists_tac ‘SUC n’ >>
+gs[listTheory.oEL_EQ_EL]
+QED
+
+Theorem transform_arg_SOME:
+!arg arg' dict.
+transform_arg dict arg = SOME arg' ==>
+SND arg = SND arg'
+Proof
+Induct >>
+rpt strip_tac >> (
+ gvs[transform_arg_def]
+)
+QED
+
+Theorem transform_args_SOME:
+!args args' dict.
+transform_args dict args = SOME args' ==>
+LENGTH args = LENGTH args' /\ MAP SND args = MAP SND args'
+Proof
+Induct >- (
+ rpt strip_tac >> (
+  gvs[transform_args_def, oFOLDR_def]
+ )
+) >>
+rpt strip_tac >> (
+ gvs[transform_args_def, oFOLDR_def]
+) >- (
+ metis_tac[]
+) >>
+metis_tac[transform_arg_SOME]
+QED
+
+Theorem transform_func_map_ALOOKUP_SOME:
+!func_map func_map' s w dict x_d_l stmt.
+dict_bij dict ==>
+ALOOKUP dict s = SOME w ==>
+transform_func_map dict func_map = SOME func_map' ==>
+ALOOKUP func_map s = SOME (stmt,x_d_l) ==>
+?stmt' w_d_l. ALOOKUP func_map' w = SOME (stmt',w_d_l) /\
+LENGTH x_d_l = LENGTH w_d_l /\
+MAP SND x_d_l = MAP SND w_d_l /\
+transform_stmt dict stmt = SOME stmt'
+Proof
+Induct >- (
+ rpt strip_tac >>
+ gvs[transform_func_map_def, oFOLDR_def]
+) >>
+rpt strip_tac >>
+PairCases_on ‘h’ >>
+gvs[transform_func_map_def, AllCaseEqs()] >- (
+ gvs[oFOLDR_def, transform_func_def] >>
+ metis_tac[transform_args_SOME]
+) >>
+gvs[oFOLDR_def, transform_func_def] >>
+‘x' ≠ w’ by (
+ metis_tac[dict_bij_injectivity]
+) >>
+gs[] >>
+first_x_assum irule >>
+gs[] >>
+metis_tac[]
+QED
+
+Theorem transform_func_map_ALOOKUP_NONE:
+!func_map func_map' s w dict x_d_l.
+dict_bij dict ==>
+ALOOKUP dict s = SOME w ==>
+transform_func_map dict func_map = SOME func_map' ==>
+ALOOKUP func_map s = NONE ==>
+ALOOKUP func_map' w = NONE
+Proof
+Induct >- (
+ rpt strip_tac >>
+ gvs[transform_func_map_def, oFOLDR_def]
+) >>
+rpt strip_tac >>
+PairCases_on ‘h’ >>
+rename1 ‘(func_name, (stmt, args))::func_map_tail’ >>
+gvs[transform_func_map_def] >>
+Cases_on ‘ALOOKUP dict func_name’ >- (
+ gvs[oFOLDR_def, transform_func_def, AllCaseEqs()]
+) >>
+rename1 ‘ALOOKUP dict func_name = SOME func_word’ >>
+Cases_on ‘transform_stmt dict stmt’ >- (
+ gvs[oFOLDR_def, transform_func_def, AllCaseEqs()]
+) >>
+Cases_on ‘transform_args dict args’ >- (
+ gvs[oFOLDR_def, transform_func_def, AllCaseEqs()]
+) >>
+rename1 ‘transform_stmt dict stmt = SOME stmt'’ >>
+rename1 ‘transform_args dict args = SOME args'’ >>
+gvs[oFOLDR_def, transform_func_def] >>
+gvs[alistTheory.ALOOKUP_def] >>
+Cases_on ‘w = func_word’ >- (
+ ‘ALOOKUP dict s = SOME w ∧ ALOOKUP dict func_name = SOME func_word ∧ s ≠ func_name’ by gvs[] >>
+ ‘w ≠ func_word’ by (
+  metis_tac[dict_bij_injectivity]
+ ) >>
+ gvs[]
+) >>
+(* Use induction hypothesis *)
+metis_tac[]
+QED
+
+(* TODO: ext_map transformation will have to be done more guardedly:
+ * Probably, check that old parameter lengths and directions agree with
+ * the hard-coded new map, otherwise return NONE. *)
+Theorem transform_ext_map_ALOOKUP_SOME:
+!ext_map ext_map' s w dict inst funs x_d_l stmt.
+ALOOKUP dict s = SOME w ==>
+transform_ext_map dict ext_map = SOME ext_map' ==>
+ALOOKUP ext_map s = SOME (SOME (x_d_l, inst), funs) ==>
+?inst' funs' w_d_l. ALOOKUP ext_map' w = SOME (SOME (w_d_l, inst'), funs') /\
+LENGTH x_d_l = LENGTH w_d_l /\
+MAP SND x_d_l = MAP SND w_d_l
+Proof
+Induct >- (
+ rpt strip_tac >>
+ gvs[transform_ext_map_def, oFOLDR_def]
+) >>
+rpt strip_tac >>
+PairCases_on ‘h’ >>
+gvs[transform_ext_map_def, AllCaseEqs()] >- (
+ first_x_assum irule >>
+ qexistsl_tac [‘dict’, ‘funs’, ‘inst’, ‘h0’] >>
+ gs[] >>
+ cheat
+) >>
+first_x_assum irule >>
+qexistsl_tac [‘dict’, ‘funs’, ‘inst’, ‘s’] >>
+gs[]
+QED
+
+(* TODO: ext_map transformation will have to be done more guardedly:
+ * Probably, check that old parameter lengths and directions agree with
+ * the hard-coded new map, otherwise return NONE. *)
+Theorem transform_ext_map_fun_ALOOKUP_SOME:
+!s1 w1 s2 w2 dict construct_info funs fun_x_d_l ext_map ext_map' ext_fun_map fun.
+ALOOKUP dict s1 = SOME w1 ==>
+ALOOKUP dict s2 = SOME w2 ==>
+transform_ext_map dict ext_map = SOME ext_map' ==>
+ALOOKUP ext_map s1 = SOME (construct_info, funs) ==>
+ALOOKUP ext_fun_map s2 = SOME (fun_x_d_l,fun) ==>
+?construct_info' funs' w_d_l fun'. ALOOKUP ext_map' w1 = SOME (construct_info', funs') /\
+ ALOOKUP funs' w2 = SOME (w_d_l, fun') /\
+LENGTH fun_x_d_l = LENGTH w_d_l /\
+MAP SND fun_x_d_l = MAP SND w_d_l
+Proof
+cheat
+QED
+
+(* TODO: If function can be looked up in regular sem, it can also be looked up in
+ * cake_sem, with same length of args. *)
+Theorem transform_ectx_lookup_funn_sig_body:
+!stmt x_d_l dict funn f ext_map func_map b_func_map e_ctx0 e_ctx1 e_ctx2.
+dict_bij dict ==>
+ transform_ectx dict (ext_map,func_map,b_func_map) =
+        SOME (e_ctx0,e_ctx1,e_ctx2) ==>
+transform_funn dict funn = SOME f ==>
+lookup_funn_sig_body funn func_map b_func_map ext_map = SOME (stmt,x_d_l) ==>
+?stmt' w_d_l. lookup_funn_sig_body' f e_ctx1 e_ctx2 e_ctx0 = SOME (stmt', w_d_l) /\
+LENGTH x_d_l = LENGTH w_d_l /\
+MAP SND x_d_l = MAP SND w_d_l /\
+transform_stmt dict stmt = SOME stmt'
+Proof
+rpt strip_tac >>
+gvs[transform_ectx_def, AllCaseEqs()] >>
+Cases_on ‘funn’ >> (
+ gvs[transform_funn_def, lookup_funn_sig_body_def, lookup_funn_sig_body'_def, AllCaseEqs()]
+) >- (
+ ‘?stmt' w_d_l. ALOOKUP e_ctx1 word' = SOME (stmt', w_d_l) /\
+  LENGTH x_d_l = LENGTH w_d_l /\ MAP SND x_d_l = MAP SND w_d_l /\
+  transform_stmt dict stmt = SOME stmt'’ by (
+  metis_tac[transform_func_map_ALOOKUP_SOME]
+ ) >>
+ qexistsl_tac [‘stmt'’, ‘w_d_l’] >>
+ metis_tac[transform_func_map_ALOOKUP_NONE]
+) >- (
+ metis_tac[transform_func_map_ALOOKUP_SOME]
+) >- (
+ simp[transform_stmt_def] >>
+ metis_tac[transform_ext_map_ALOOKUP_SOME]
+) >- (
+ simp[transform_stmt_def] >>
+ metis_tac[transform_ext_map_fun_ALOOKUP_SOME]
+)
+QED
+
+Theorem transform_e_preserves_is_arg_red:
+!e e' dict d.
+transform_e dict e = SOME e' ==>
+(is_arg_red d e <=> is_arg_red' d e')
+Proof
+(* Need to induct, since this is dependent on nested es *)
+Induct >> (
+ rpt strip_tac >>
+ imp_res_tac transform_e_subtypes >>
+ gvs[is_arg_red_def, is_arg_red'_def, is_const_def, is_const'_def, is_e_lval_def, is_e_lval'_def, get_lval_of_e_def, get_lval_of_e'_def]
+) >> (
+ Cases_on ‘is_d_out d’ >> (
+  gs[]
+ ) >>
+ qpat_x_assum ‘transform_e dict _ = SOME _’
+  (fn thm => assume_tac $ ONCE_REWRITE_RULE [transform_e_def] thm >> 
+             gvs[AllCaseEqs()])
+) >- (
+ qpat_x_assum ‘!e'''. _’
+  (fn thm => assume_tac $ Q.SPECL [‘e''’, ‘dict’, ‘d’] thm) >>
+ gs[] >>
+ Cases_on ‘get_lval_of_e e’ >> Cases_on ‘get_lval_of_e' e''’ >> (
+  gs[]
+ )
+) >>
+qpat_x_assum ‘!e' dict' d.
+         transform_e dict' e = SOME e' ==> _’
+ (fn thm => assume_tac $ Q.SPECL [‘e1'’, ‘dict’, ‘d’] thm) >>
+gs[] >>
+Cases_on ‘get_lval_of_e e’ >> Cases_on ‘get_lval_of_e' e1'’ >> (
+ gs[]
+)
+QED
+
+Theorem INDEX_FIND_preserved:
+!P P' l l' i x.
+LENGTH l = LENGTH l' ==>
+(!j. j < LENGTH l ==> (P (EL j l) <=> P' (EL j l'))) ==>
+INDEX_FIND 0 P l = SOME (i, x) ==>
+?x'. INDEX_FIND 0 P' l' = SOME (i, x')
+Proof
+rpt strip_tac >>
+‘i < LENGTH l /\ EL i l = x /\ P x /\ 
+ !j. j < i ==> ~P (EL j l)’ by (
+ imp_res_tac INDEX_FIND_EQ_SOME_0 >>
+ gs[]
+) >>
+‘i < LENGTH l'’ by gs[] >>
+qexists_tac ‘EL i l'’ >>
+simp[INDEX_FIND_EQ_SOME_0] >>
+gs[] >>
+‘P (EL i l)’ suffices_by metis_tac[] >>
+gvs[]
+QED
+
+Theorem transform_list_unred_arg_index_SOME:
+!l l' d_l i dict.
+LENGTH d_l = LENGTH l ==>
+unred_arg_index d_l l = SOME i ==>
+transform_e dict (e_list l) = SOME (e'_list l') ==>
+unred_arg_index' d_l l' = SOME i
+Proof
+rpt strip_tac >>
+gs[unred_arg_index_def, unred_arg_index'_def, find_unred_arg_def, find_unred_arg'_def, AllCaseEqs()] >>
+‘LENGTH l = LENGTH l'’ by (
+ imp_res_tac transform_list_LENGTH >>
+ fs[]
+) >>
+‘!j. j < LENGTH l ==> 
+     (is_arg_red (EL j d_l) (EL j l) <=> is_arg_red' (EL j d_l) (EL j l'))’ by (
+ rpt strip_tac >>
+ irule transform_e_preserves_is_arg_red >>
+ ‘?ej ej'. EL j l = ej /\ EL j l' = ej' /\ transform_e dict ej = SOME ej'’ by (
+   imp_res_tac transform_list_EL >>
+   qexistsl_tac [‘EL j l’, ‘EL j l'’] >>
+   fs[listTheory.oEL_EQ_EL]
+ ) >>
+ metis_tac[]
+) >>
+‘?de. INDEX_FIND 0 (\(d,e). ~is_arg_red' d e) (ZIP (d_l,l')) = SOME (i,de)’ suffices_by metis_tac[] >>
+irule (Q.ISPECL [‘(\(d,e). ~is_arg_red d e)’] INDEX_FIND_preserved) >>
+qexistsl_tac [‘ZIP(d_l, l)’, ‘de’] >>
+gvs[] >>
+rpt strip_tac >>
+(* TODO: Looks easy... *)
+Cases_on ‘EL j (ZIP(d_l, l))’ >>
+Cases_on ‘EL j (ZIP(d_l, l'))’ >>
+simp[] >>
+‘q = EL j d_l /\ q' = EL j d_l /\ r = EL j l /\ r' = EL j l'’ suffices_by metis_tac[] >>
+‘j < LENGTH l’ by gs[] >>
+‘LENGTH d_l = LENGTH l’ suffices_by (
+ rpt strip_tac >> (
+  imp_res_tac listTheory.EL_ZIP >>
+  gvs[]
+ ) >> (
+  ‘LENGTH d_l = LENGTH l'’ by gs[] >>
+  imp_res_tac listTheory.EL_ZIP >>
+  gvs[]
+ )
+) >>
+gs[]
+QED
+
+Theorem transform_list_unred_arg_index_NONE:
+!l l' d_l dict.
+LENGTH d_l = LENGTH l ==>
+unred_arg_index d_l l = NONE ==>
+transform_e dict (e_list l) = SOME (e'_list l') ==>
+unred_arg_index' d_l l' = NONE
+Proof
+cheat
+QED
+
+Theorem transform_e_call_arg:
+!l l' funn f e e' dict.
+transform_e dict (e_call funn l) = SOME $ e'_call f l' ==>
+MEM e l ==>
+?e'. transform_e dict e = SOME e'
+Proof
+Induct >- (
+ gs[listTheory.MEM]
+) >>
+rpt strip_tac >>
+qpat_x_assum ‘transform_e dict (e_call funn (h::t)) = SOME (e'_call f l')’
+ (fn thm => assume_tac $ ONCE_REWRITE_RULE [transform_e_def] thm >> 
+  gvs[AllCaseEqs()]) >>
+Cases_on ‘e = h’ >- (
+ gs[]
+) >>
+qpat_x_assum ‘!l''. _’
+ (fn thm => irule thm) >>
+gs[] >>
+qexistsl_tac [‘f’, ‘funn’, ‘t'’] >>
+simp[Once transform_e_def, AllCaseEqs()] >>
+Cases_on ‘l’ >> Cases_on ‘t'’ >> (
+ gs[listTheory.MEM]
+) >> (
+qpat_x_assum ‘transform_e dict (e_list (h'::t)) = SOME _’
+ (fn thm => assume_tac $ ONCE_REWRITE_RULE [transform_e_def] thm >> 
+  gvs[AllCaseEqs()])
+)
+QED
+
+Theorem transform_e_call_LUPDATE:
+!l l' funn f ei ei' i dict.
+transform_funn dict funn = SOME f ==>
+transform_e dict (e_list l) = SOME (e'_list l') ==>
+transform_e dict ei = SOME ei' ==>
+transform_e dict (e_call funn (LUPDATE ei i l)) = SOME $ e'_call f (LUPDATE ei' i l')
+Proof
+Induct >- (
+ rpt strip_tac >>  
+ gs[listTheory.LUPDATE_def] >>
+ ‘l' = []’ by gs[Once transform_e_def] >>
+ simp[Once transform_e_def]
+) >>
+rpt strip_tac >>
+qpat_x_assum ‘transform_e dict (e_list (h::t)) = SOME (e'_list l')’
+ (fn thm => assume_tac $ ONCE_REWRITE_RULE [transform_e_def] thm >> 
+            gvs[AllCaseEqs()]) >>
+Cases_on ‘i’ >- (
+ gs[listTheory.LUPDATE_def] >>
+ simp[Once transform_e_def]
+) >>
+gs[listTheory.LUPDATE_def] >>
+simp[Once transform_e_def] >>
+qexists_tac ‘e'_list (LUPDATE ei' n t')’ >>
+simp[] >>
+‘transform_e dict (e_call funn (LUPDATE ei n l)) = SOME (e'_call f (LUPDATE ei' n t'))’ suffices_by (
+ rpt strip_tac >>
+ qpat_x_assum ‘transform_e dict (e_call funn (LUPDATE ei n l)) =
+                SOME (e'_call f (LUPDATE ei' n t'))’
+  (fn thm => assume_tac $ ONCE_REWRITE_RULE [transform_e_def] thm >> 
+             gvs[AllCaseEqs()]) >> (
+  simp[listTheory.LUPDATE_def, Once transform_e_def]
+ )
+) >>
+first_x_assum irule >>
+gs[]
+QED
+
+(* Describes how copyin behaviour is preserved over translation *)
+Theorem transform_scope_copyin:
+transform_ectx dict (ext_map,func_map,b_func_map) = SOME (e_ctx0,e_ctx1,e_ctx2) ==>
+transform_scope_list dict g_scope_list = SOME g_scope_list' ==>
+transform_scope_list dict scope_list = SOME scope_list' ==>
+lookup_funn_sig_body funn func_map b_func_map ext_map = SOME (stmt,x_d_l) ==>
+copyin_exec uninit_zero (MAP FST x_d_l) (MAP SND x_d_l) (h::t) g_scope_list scope_list = SOME scope ==>
+transform_scope dict scope = SOME res'' ==>
+lookup_funn_sig_body' f e_ctx1 e_ctx2 e_ctx0 = SOME (res',x_d_l') ==>
+copyin' (MAP FST x_d_l') (MAP SND x_d_l') (e'::t') g_scope_list' scope_list' = SOME res''
+Proof
+cheat
+QED
+
+Theorem e_exec'_completeness_call:
+!f l.
+l_complete l ==>
+e_exec'_complete (e'_call f l)
+Proof
+gs[e_exec'_complete_def] >>
+rpt strip_tac >>
+PairCases_on ‘e_ctx’ >>
+qpat_x_assum ‘transform_e dict e1 = SOME (e'_call f l)’ (fn thm => assume_tac $ ONCE_REWRITE_RULE [transform_e_def] thm >> gvs[listTheory.UNZIP_MAP, AllCaseEqs()]) >- (
+ (* Case: No args - then no args can also be unreduced *)
+ gvs[p4_exec_semTheory.e_exec_def, unred_arg_index_def, find_unred_arg_def, listTheory.INDEX_FIND_def, transform_frame_list_def, oFOLDR_def, AllCaseEqs()] >>
+ (* TODO: The new frame needs to be properly resolved... *)
+ gvs[e_exec'_def, p4_exec_semTheory.e_exec_def, AllCaseEqs()] >>
+‘?v1. lookup_funn_sig_body' f e_ctx1 e_ctx2 e_ctx0 = SOME v1 /\
+ ?stmt'. v1 = (stmt', []) /\ transform_stmt dict stmt = SOME stmt'’ by (
+  imp_res_tac transform_ectx_lookup_funn_sig_body >>
+  qexists_tac ‘(stmt',[])’ >>
+  gs[] >>
+  metis_tac[transform_list_LENGTH]
+ ) >> gvs[] >>
+ gvs[unred_arg_index'_def, find_unred_arg'_def, listTheory.INDEX_FIND_def, copyin'_def, all_arg_update_for_newscope'_def, transform_e_def, transform_varn_def, transform_frame_def, transform_scope_list_def, p4_exec_semTheory.copyin_exec_def, p4_exec_semTheory.all_arg_update_for_newscope_exec_def, transform_scope_def, oFOLDR_def, AllCaseEqs()]
+) >>
+(* Case: Args *)
+gvs[e_exec'_def, p4_exec_semTheory.e_exec_def, AllCaseEqs()] >- (
+ (* Fully reduced *)
+ gvs[transform_frame_list_def, transform_frame_def, oFOLDR_def] >>
+‘?v1. lookup_funn_sig_body' f e_ctx1 e_ctx2 e_ctx0 = SOME v1 /\
+ ?stmt' x_d_l. v1 = (stmt', x_d_l) /\ LENGTH x_d_l = SUC (LENGTH t') /\ transform_stmt dict stmt = SOME stmt'’ by (
+  imp_res_tac transform_ectx_lookup_funn_sig_body >>
+  qexists_tac ‘(stmt',w_d_l)’ >>
+  gs[] >>
+  metis_tac[transform_list_LENGTH]
+ ) >> gvs[] >>
+ (* TODO: Do nicer *)
+ ‘unred_arg_index' (MAP SND x_d_l') (e'::t') = NONE’ by (
+  irule transform_list_unred_arg_index_NONE >>
+  qexistsl_tac [‘dict’, ‘h::t’] >>
+  imp_res_tac transform_list_LENGTH >>
+  gs[] >>
+  simp[transform_e_def] >>
+  ‘MAP SND x_d_l' = MAP SND x_d_l’ by (
+   imp_res_tac transform_ectx_lookup_funn_sig_body >>
+   gvs[]
+  ) >>
+  gs[]
+ ) >>
+ gs[] >>
+ qpat_x_assum ‘transform_e dict (e_var (varn_star funn)) = SOME e'2’ (fn thm => assume_tac $ ONCE_REWRITE_RULE [transform_e_def] thm >> gvs[AllCaseEqs()]) >>
+ qpat_x_assum ‘transform_scope_list dict [scope] = SOME scope_list''’ (fn thm => assume_tac $ ONCE_REWRITE_RULE [transform_scope_list_def] thm >> gvs[AllCaseEqs()]) >>
+ gvs[transform_varn_def, oFOLDR_def] >>
+ metis_tac[transform_scope_copyin]
+) >>
+‘?v1. lookup_funn_sig_body' f e_ctx1 e_ctx2 e_ctx0 = SOME v1 /\
+ ?stmt' x_d_l'.
+  v1 = (stmt', x_d_l') /\ LENGTH x_d_l' = SUC (LENGTH t') /\ MAP SND x_d_l = MAP SND x_d_l'’ by (
+  imp_res_tac transform_ectx_lookup_funn_sig_body >>
+  qexists_tac ‘(stmt',w_d_l)’ >>
+  gs[] >>
+  metis_tac[transform_list_LENGTH]
+ ) >> gvs[] >>
+‘unred_arg_index' (MAP SND x_d_l') (e'::t') = SOME i’ by (
+ irule transform_list_unred_arg_index_SOME >>
+ qexistsl_tac [‘dict’, ‘h::t’] >>
+ gs[] >>
+ simp[Once transform_e_def] >>
+ metis_tac[transform_list_LENGTH]
+) >> gs[] >>
+‘?ei. EL i (h::t) = ei’ by metis_tac[unred_arg_index_in_range] >>
+‘?e'i. oEL i (e'::t') = SOME e'i’ by (
+ imp_res_tac unred_arg_index_in_range >>
+ imp_res_tac oEL_SOME >>
+ imp_res_tac transform_list_LENGTH >>
+ ‘i < LENGTH (e'::t')’ suffices_by metis_tac[oEL_SOME] >>
+ gvs[]
+) >> gs[] >>
+‘?e''i. transform_e dict e'' = SOME e''i’ by (
+ (* TODO: Do before? *)
+ imp_res_tac transform_e_subtypes >>
+ gvs[] >>
+ irule transform_e_call_arg >>
+ qexistsl_tac [‘funn'’, ‘funn’, ‘(LUPDATE e'' i (h::t))’, ‘l''’] >>
+ gs[listTheory.MEM_LUPDATE, listTheory.oEL_EQ_EL] >>
+ imp_res_tac oEL_SOME >>
+ metis_tac[transform_list_LENGTH]
+) >>
+qexists_tac ‘(e''i, frame_list')’ >>
+CONJ_TAC >- (
+ (* Use induction hypothesis on the ith position *)
+ ‘e_exec'_complete e'i’ by (
+  metis_tac[l_complete_mem, listTheory.MEM_EL, listTheory.oEL_EQ_EL]
+ ) >>
+ gs[e_exec'_complete_def] >>
+ ‘!e1.
+   transform_e dict e1 = SOME e'i ==>
+   !tbl_map pars_map frame_list e2 apply_table_f.
+     e_exec uninit_zero
+       (apply_table_f,ext_map,func_map,b_func_map,pars_map,tbl_map)
+       g_scope_list scope_list e1 =
+     SOME (e2,frame_list) ==>
+     !e'2.
+       transform_e dict e2 = SOME e'2 ==>
+       !frame_list'.
+         transform_frame_list dict frame_list = SOME frame_list' ==>
+         e_exec' (e_ctx0,e_ctx1,e_ctx2) g_scope_list' scope_list' e'i =
+         SOME (e'2,frame_list')’ by (
+  res_tac
+ ) >>
+ qpat_x_assum ‘!e1 dict. _’ (fn thm => ALL_TAC) >>
+ qpat_x_assum ‘!e1. _’ (fn thm => irule thm) >>
+ qexistsl_tac [‘apply_table_f’, ‘ei’, ‘e''’, ‘frame_list’, ‘pars_map’, ‘tbl_map’] >>
+ gs[] >>
+ irule transform_list_EL >>
+ qexistsl_tac [‘i’, ‘h::t’, ‘e'::t'’] >>
+ gs[listTheory.oEL_EQ_EL] >>
+ simp[Once transform_e_def] >>
+ metis_tac[transform_list_LENGTH]
+) >>
+qexists_tac ‘e''i’ >>
+gvs[] >>
+‘transform_e dict (e_call funn (LUPDATE e'' i (h::t))) = SOME $ e'_call f (LUPDATE e''i i (e'::t'))’ by (
+ irule transform_e_call_LUPDATE >>
+ gs[] >>
+ simp[Once transform_e_def]
+) >>
+gvs[]
+QED
+
+(* TODO: Change form, only use e_struct l? *)
+(* Proof similar to transform_list_unred_arg_index_SOME *)
+Theorem transform_struct_unred_mem_index_NONE:
+!t t' e e' dict.
+unred_mem_index (e::MAP SND t) = NONE ==>
+transform_e dict e = SOME e' ==>
+transform_e dict (e_struct t) = SOME (e'_struct t') ==>
+unred_mem_index' (e'::MAP_SND t') = NONE
+Proof
+cheat
+(*
+Induct >> (
+ rpt strip_tac >>
+ gvs[Once transform_e_def, MAP_SND_EQ, unred_mem_index'_def, unred_mem'_def, listTheory.INDEX_FIND_def, is_const'_def, AllCaseEqs()]
+) >> (
+ qpat_x_assum ‘transform_e dict (e_struct _) = SOME _’ (fn thm => assume_tac $ ONCE_REWRITE_RULE [transform_e_def] thm >> gvs[AllCaseEqs()]) >>
+ gvs[listTheory.INDEX_FIND_def, is_const'_def, unred_mem_index_def, unred_mem_def, is_const_def, AllCaseEqs()]
+) >>
+gs[AllCaseEqs()]
+)
+*)
+QED
+
+(* TODO: Change form, only use e_struct l? *)
+(* Proof similar to transform_list_unred_arg_index_NONE *)
+Theorem transform_struct_unred_mem_index_SOME:
+!e e' t t' i dict.
+unred_mem_index (e::MAP SND t) = SOME i ==>
+transform_e dict e = SOME e' ==>
+transform_e dict (e_struct t) = SOME (e'_struct t') ==>
+unred_mem_index' (e'::MAP_SND t') = SOME i
+Proof
+cheat
+QED
+
+(* Relates e and v transformations of structs *)
+(* TODO: What if the expressions in the struct are not values? *)
+Theorem transform_e_v_struct:
+!t t' t'' dict.
+transform_e dict (e_struct t) = SOME (e'_struct t') ==>
+transform_v dict
+          (v_struct (ZIP (MAP FST t,MAP (\e. THE (v_of_e e)) (MAP SND t)))) =
+        SOME (v'_struct t'') ==>
+vl_of_el' (MAP_SND t') = SOME (MAP SND t'') /\
+        ZIP (MAP_FST t',MAP SND t'') = t''
+Proof
+cheat
+QED
+
+Theorem transform_e_struct_LENGTH:
+!t t' dict.
+transform_e dict (e_struct t) = SOME (e'_struct t') ==>
+LENGTH t = LENGTH t'
+Proof
+Induct >> (
+ rpt strip_tac >>
+ gs[Once transform_e_def, AllCaseEqs()]
+) >>
+qpat_x_assum ‘transform_e dict (e_struct _) = SOME _’ (fn thm => assume_tac $ ONCE_REWRITE_RULE [transform_e_def] thm >> gvs[AllCaseEqs()]) >>
+qpat_x_assum ‘!t'' dict'. _’ (fn thm => irule thm) >>
+qexists_tac ‘dict’ >>
+Cases_on ‘t’ >> Cases_on ‘t''’ >> (
+ gs[]
+) >> (
+qpat_x_assum ‘transform_e dict (e_struct _) = SOME _’ (fn thm => assume_tac $ ONCE_REWRITE_RULE [transform_e_def] thm >> gvs[AllCaseEqs()])
+)
+QED
+
+(* TODO: Fix *)
+Theorem MAP_SND_EQUIV:
+!l.
+MAP_SND l = MAP SND l
+Proof
+gs[p4_cake_exec_semTheory.MAP_SND_EQ]
+QED
+
+(* TODO: Fix *)
+Theorem MAP_FST_EQUIV:
+!l.
+MAP_FST l = MAP FST l
+Proof
+gs[p4_cake_exec_semTheory.MAP_FST_EQ]
+QED
+
+(* TODO: Formulate in a nicer way *)
+Theorem struct_lemma:
+transform_e dict (e_struct t) = SOME (e'_struct t') ==>
+transform_e dict (e_struct t'') = SOME (e'_struct t'3') ==>
+transform_e dict e'3' = SOME e'2 ==>
+transform_e dict e'4' = SOME e'5'==>
+ALOOKUP dict x = SOME x' ==>
+ZIP (x::MAP FST t,LUPDATE e'3' i (e'::MAP SND t)) = (x,e'4')::t'' ==>
+ZIP (x'::MAP FST t',LUPDATE e'2 i (e''::MAP SND t')) = (x',e'5')::t'3'
+Proof
+cheat
+QED
+
+Theorem e_exec'_completeness_struct:
+!l.
+w_e_l_exec'_complete l ==>
+e_exec'_complete (e'_struct l)
+Proof
+gs[e_exec'_complete_def] >>
+rpt strip_tac >>
+(* 1. Rewrite transformation of initial state *)
+qpat_x_assum ‘transform_e dict e1 = SOME (e'_struct l)’ (fn thm => assume_tac $ ONCE_REWRITE_RULE [transform_e_def] thm >> gvs[listTheory.UNZIP_MAP, AllCaseEqs()]) >- (
+ (* Case: empty struct *)
+ (* 2. Rewrite execution *)
+ gvs[p4_exec_semTheory.e_exec_def, e_exec'_def, AllCaseEqs()] >> (
+ gvs[transform_frame_list_def, oFOLDR_def]
+) >- (  
+  gs[vl_of_el'_def, vl_of_el_def, MAP_SND_def, MAP_FST_def, AllCaseEqs()] >>
+  gvs[AllCaseEqs(), transform_e_def, transform_v_def] >>
+  metis_tac[unred_mem_index_same]
+ ) >>
+ gvs[unred_mem_index_def, unred_mem_def, listTheory.INDEX_FIND_def, AllCaseEqs()]
+) >>
+(* Case: non-empty struct *)
+gvs[p4_exec_semTheory.e_exec_def, e_exec'_def, AllCaseEqs()] >- (
+ (* No unreduced fields *)
+ DISJ1_TAC >>
+ gs[vl_of_el'_def, vl_of_el_def, MAP_SND_def, MAP_FST_def, AllCaseEqs()] >>
+ (* From unred_mem_index *)
+ imp_res_tac unred_mem_index_NONE >>
+ gs[is_consts_def] >>
+ Cases_on ‘e'’ >> (gs[is_const_def]) >>
+ gvs[Once transform_e_def, listTheory.UNZIP_MAP, AllCaseEqs()] >>
+ gvs[v_of_e_def, MAP_SND_def, MAP_FST_def, vl_of_el'_def, Once transform_v_def, AllCaseEqs()] >>
+ CONJ_TAC >- (
+  (* Ok *)
+  metis_tac[transform_struct_unred_mem_index_NONE]
+ ) >>
+ qpat_x_assum ‘transform_e dict (e_v v) = SOME e''’ (fn thm => assume_tac $ ONCE_REWRITE_RULE [transform_e_def] thm >> gvs[listTheory.UNZIP_MAP, AllCaseEqs()]) >>
+ gs[v_of_e'_def] >>
+ qexists_tac ‘v''::MAP SND t''’ >>
+ gvs[transform_frame_list_def, oFOLDR_def] >>
+ metis_tac[transform_e_v_struct]
+) >>
+DISJ2_TAC >>
+gs[w_e_l_exec'_complete_def] >>
+gs[l_complete_def] >>
+qexists_tac ‘i’ >>
+CONJ_TAC >- (
+ gvs[MAP_SND_def] >>
+ metis_tac[transform_struct_unred_mem_index_SOME]
+) >>
+‘?e. SOME e = oEL i (e''::MAP SND t')’ by (
+ imp_res_tac unred_mem_index_in_range >>
+ imp_res_tac oEL_SOME >>
+ imp_res_tac transform_e_struct_LENGTH >>
+ ‘i < LENGTH (e''::MAP SND t')’ suffices_by metis_tac[oEL_SOME] >>
+ gvs[]
+) >>     
+res_tac >>
+qexists_tac ‘e’ >>
+CONJ_TAC >- (
+ gvs[p4_cake_exec_semTheory.MAP_SND_def, MAP_SND_EQUIV]
+) >>
+qpat_x_assum ‘transform_e dict
+          (e_struct (ZIP (x::MAP FST t,LUPDATE e'³' i (e'::MAP SND t)))) =
+        SOME e'2’ (fn thm => ASSUME_TAC $ ONCE_REWRITE_RULE [transform_e_def] thm >> gvs[listTheory.UNZIP_MAP, listTheory.ZIP_EQ_NIL, AllCaseEqs()]) >>
+gs[e_exec'_complete_def] >>
+‘!e1.
+ transform_e dict e1 = oEL i (e''::MAP SND t') ==>
+ !tbl_map pars_map frame_list e2 apply_table_f.
+   e_exec uninit_zero
+     (apply_table_f,ext_map,func_map,b_func_map,pars_map,tbl_map)
+     g_scope_list scope_list e1 =
+   SOME (e2,frame_list) ==>
+   !e'2.
+     transform_e dict e2 = SOME e'2 ==>
+     !frame_list'.
+       transform_frame_list dict frame_list = SOME frame_list' ==>
+       e_exec' e_ctx g_scope_list' scope_list' e =
+       SOME (e'2,frame_list')’ by (
+ res_tac
+) >>
+(* More fiddling needed *)
+qpat_x_assum ‘!e1.
+          transform_e dict e1 = oEL i (e''::MAP SND t') ==>
+          !tbl_map pars_map frame_list e2 apply_table_f.
+            e_exec uninit_zero
+              (apply_table_f,ext_map,func_map,b_func_map,pars_map,tbl_map)
+              g_scope_list scope_list e1 =
+            SOME (e2,frame_list) ==>
+            !e'2.
+              transform_e dict e2 = SOME e'2 ==>
+              !frame_list'.
+                transform_frame_list dict frame_list = SOME frame_list' ==>
+                e_exec' e_ctx g_scope_list' scope_list' e =
+                SOME (e'2,frame_list')’ (fn thm => ASSUME_TAC $ Q.SPECL [‘EL i (e'::MAP SND (t:(string # e) list))’] thm >> gs[]) >>
+(* TODO: Why? *)
+‘transform_e dict (EL i (e'::MAP SND t)) = oEL i (e''::MAP SND t')’ by cheat >>
+gvs[] >>
+‘!e'2.
+          transform_e dict e'3' = SOME e'2 ==>
+          !frame_list'.
+            transform_frame_list dict frame_list = SOME frame_list' ==>
+            e_exec' e_ctx g_scope_list' scope_list' e =
+            SOME (e'2,frame_list')’ by (
+ res_tac
+) >>
+(* TODO: Why? *)
+‘?e'2. transform_e dict e'3' = SOME e'2’ by cheat >>
+gvs[MAP_FST_EQUIV, MAP_SND_EQUIV] >>
+qpat_x_assum ‘!e1. _ ’ (fn thm => ALL_TAC) >>
+qpat_x_assum ‘!e1. _ ’ (fn thm => ALL_TAC) >>
+qpat_x_assum ‘!e1. _ ’ (fn thm => ALL_TAC) >>
+(* TODO: Why? *)
+‘x = x''’ by cheat >> gvs[] >>
+irule struct_lemma >>
+qexistsl_tac [‘dict’, ‘e'’, ‘e'3'’, ‘e'4'’, ‘t’, ‘t''’, ‘x’] >>
+gs[]
+QED
+
+Theorem e_exec'_completeness_binop:
+!e b e0.
+e_exec'_complete e ==>
+e_exec'_complete e0 ==>
+e_exec'_complete (e'_binop e b e0)
+Proof
+gs[e_exec'_complete_def] >>
+rpt strip_tac >>
+(* 1. Rewrite transformation of initial state *)
+qpat_x_assum ‘transform_e dict e1 = SOME (e'_binop e b e0)’ (fn thm => ASSUME_TAC $ ONCE_REWRITE_RULE [transform_e_def] thm >> gvs[listTheory.UNZIP_MAP, AllCaseEqs()]) >>
+(* 2. Rewrite execution *)
+qpat_x_assum ‘e_exec uninit_zero
+         (apply_table_f,ext_map,func_map,b_func_map,pars_map,tbl_map)
+         g_scope_list scope_list (e_binop e1' b e2') =
+       SOME (e2,frame_list)’ (fn thm => ASSUME_TAC $ ONCE_REWRITE_RULE [p4_exec_semTheory.e_exec_def] thm >> simp[e_exec'_def] >> gvs[listTheory.UNZIP_MAP, AllCaseEqs()]) >> (
+ gvs[transform_frame_list_def, oFOLDR_def] >>
+ imp_res_tac transform_e_subtypes >>
+ imp_res_tac transform_e_is_v >>
+ imp_res_tac transform_e_not_is_v >>
+ gvs[]
+) >- (
+ (* Non-recursive case: Short-circuit *)
+ Cases_on ‘v’ >> Cases_on ‘b’ >> (
+  gs[p4_exec_semTheory.e_exec_short_circuit_def]
+ ) >- (
+  qpat_x_assum ‘transform_e dict (e_v (v_bool b')) = SOME (e'_v v')’ (fn thm => ASSUME_TAC $ ONCE_REWRITE_RULE [transform_e_def] thm >> gvs[AllCaseEqs()] >> gs[transform_v_def]) >>
+  Cases_on ‘b'’ >> (
+   gvs[p4_exec_semTheory.e_exec_short_circuit_def, e_exec_short_circuit'_def] >>
+   qpat_x_assum ‘transform_e dict (e_v (v_bool F)) = SOME e'2’ (fn thm => ASSUME_TAC $ ONCE_REWRITE_RULE [transform_e_def] thm >> gvs[AllCaseEqs()] >> gs[transform_v_def])
+  )
+ ) >>
+ qpat_x_assum ‘transform_e dict (e_v (v_bool b')) = SOME (e'_v v')’ (fn thm => ASSUME_TAC $ ONCE_REWRITE_RULE [transform_e_def] thm >> gvs[AllCaseEqs()] >> gs[transform_v_def]) >>
+ Cases_on ‘b'’ >> (
+  gvs[p4_exec_semTheory.e_exec_short_circuit_def, e_exec_short_circuit'_def] >>
+  qpat_x_assum ‘transform_e dict (e_v (v_bool T)) = SOME e'2’ (fn thm => ASSUME_TAC $ ONCE_REWRITE_RULE [transform_e_def] thm >> gvs[AllCaseEqs()] >> gs[transform_v_def])
+ )
+) >- (
+ (* Non-recursive case *)
+ qpat_x_assum ‘!e1. _’ (fn thm => ALL_TAC) >>
+ qpat_x_assum ‘!e1. _’ (fn thm => ALL_TAC) >>
+ (* TODO: Bitwidth issue *)
+ Cases_on ‘e2'’ >> (
+  gvs[p4_exec_semTheory.is_v_def]
+ ) >>
+ Cases_on ‘e0’ >> (
+  gvs[is_v'_def]
+ ) >>
+ fs[Once transform_e_def] >>
+ Cases_on ‘b’ >> Cases_on ‘v’ >> Cases_on ‘v''''’ >> (
+  gvs[p4_exec_semTheory.binop_exec_def, p4_exec_semTheory.e_exec_binop_def, e_exec_binop'_def, AllCaseEqs()]
+ ) >> (
+  fs[Once transform_v_def] >>
+  gvs[] >>
+  gs[binop_exec'_def, AllCaseEqs()] >>
+  Cases_on ‘p’ >> Cases_on ‘p'’ >> (
+   gs[bitv_binop_def, bitv_binop'_def, get_bitv_binop'_def, AllCaseEqs()]
+  )
+ ) >>
+ (* TODO: Bitwidth problem *)
+ cheat
+) >- (
+ (* Recursive: 2nd arg red *)
+ qpat_x_assum ‘transform_e dict (e_binop (e_v v) b e2'') = SOME (e'_binop e1' b e2'³')’ (fn thm => ASSUME_TAC $ ONCE_REWRITE_RULE [transform_e_def] thm >> gvs[AllCaseEqs()]) >>
+ metis_tac[]
+) >> (
+ (* Recursive cases *)
+ qpat_x_assum ‘transform_e dict (e_binop e1'' b e2') = SOME (e'_binop _ b _)’ (fn thm => ASSUME_TAC $ ONCE_REWRITE_RULE [transform_e_def] thm >> gvs[AllCaseEqs()]) >>
+ metis_tac[]
+)
+QED
+
+Theorem e_exec'_completeness_concat:
+!e e0.
+e_exec'_complete e ==>
+e_exec'_complete e0 ==>
+e_exec'_complete (e'_concat e e0)
+Proof
+gs[e_exec'_complete_def] >>
+rpt strip_tac >>
+(* 1. Rewrite transformation of initial state *)
+qpat_x_assum ‘transform_e dict e1 = SOME (e'_concat e e0)’ (fn thm => ASSUME_TAC $ ONCE_REWRITE_RULE [transform_e_def] thm >> gvs[listTheory.UNZIP_MAP, AllCaseEqs()]) >>
+(* 2. Rewrite execution *)
+gvs[e_exec'_def, p4_exec_semTheory.e_exec_def, AllCaseEqs()] >- (
+ gvs[transform_frame_list_def, oFOLDR_def] >>
+ qpat_x_assum ‘!e1. _’ (fn thm => ALL_TAC) >>
+ qpat_x_assum ‘!e1. _’ (fn thm => ALL_TAC) >>
+ (* Case 2a: e1' and e2' are both values *)
+ ‘is_v_bit' e’ by metis_tac[transform_e_is_v_bit] >> gs[] >>
+ ‘is_v_bit' e0’ by metis_tac[transform_e_is_v_bit] >> gs[] >>
+ (* First, get result of operation on cake_sem in proof goal *)
+ Cases_on ‘e’ >> (gs[is_v_bit'_def]) >>
+ Cases_on ‘e0’ >> (gs[is_v_bit'_def]) >>
+ Cases_on ‘v'’ >> (gs[is_v_bit'_def]) >>
+ Cases_on ‘v''’ >> (gs[is_v_bit'_def]) >>
+ simp[e_exec_concat'_def] >>
+ (* Then, obtain everything involved
+  * in the operation from regular semantics by case analysis *)
+ Cases_on ‘e1'’ >> (gs[p4_exec_semTheory.is_v_bit_def]) >>
+ Cases_on ‘e2'’ >> (gs[p4_exec_semTheory.is_v_bit_def]) >>
+ Cases_on ‘v'’ >> (gs[p4_exec_semTheory.is_v_bit_def]) >>
+ Cases_on ‘v''’ >> (gs[p4_exec_semTheory.is_v_bit_def]) >>
+ (* Apply regular operation *)
+ gvs[p4_exec_semTheory.e_exec_concat_def] >>
+ (* Connect the concrete values via translation *)
+ gvs[transform_e_def, transform_v_def]
+) >- (
+ (* Case 2b: e2' is not value *)
+ ‘is_v_bit' e’ by metis_tac[transform_e_is_v_bit] >> gs[] >>
+ ‘~is_v_bit' e0’ by metis_tac[transform_e_not_is_v_bit] >> gs[] >>
+ (* 3. Rewrite transformation of final state *)
+ qpat_x_assum ‘transform_e dict (e_concat e1' e2'') = SOME e'2’ (fn thm => ASSUME_TAC $ ONCE_REWRITE_RULE [transform_e_def] thm >> gvs[app_opt_def, AllCaseEqs()]) >>
+ (* 4. Use induction hypothesis *)
+ metis_tac[]
+) >>
+‘~is_v_bit' e’ by metis_tac[transform_e_not_is_v_bit] >> gs[] >>
+(* 3. Rewrite transformation of final state *)
+qpat_x_assum ‘transform_e dict (e_concat e1'' e2') = SOME e'2’ (fn thm => ASSUME_TAC $ ONCE_REWRITE_RULE [transform_e_def] thm >> gvs[app_opt_def, AllCaseEqs()]) >>
+(* 4. Use induction hypothesis *)
+metis_tac[]
+QED
+
+Theorem e_exec'_completeness_slice:
+!e e0 e1.
+e_exec'_complete e ==>
+e_exec'_complete e0 ==>
+e_exec'_complete e1 ==>
+e_exec'_complete (e'_slice e e0 e1)
+Proof
+gs[e_exec'_complete_def] >>
+rpt strip_tac >>
+(* 1. Rewrite transformation of initial state *)
+qpat_x_assum ‘transform_e dict e1' = SOME (e'_slice e e0 e1)’ (fn thm => ASSUME_TAC $ ONCE_REWRITE_RULE [transform_e_def] thm >> gvs[listTheory.UNZIP_MAP, AllCaseEqs()]) >>
+(* 2. Rewrite execution *)
+gvs[e_exec'_def, p4_exec_semTheory.e_exec_def, AllCaseEqs()] >- (
+ (* Case 2a: e1'', e2'' and e3 are all values *)
+ gvs[transform_frame_list_def, oFOLDR_def] >>
+ qpat_x_assum ‘!e1. _’ (fn thm => ALL_TAC) >>
+ qpat_x_assum ‘!e1. _’ (fn thm => ALL_TAC) >>
+ qpat_x_assum ‘!e1'. _’ (fn thm => ALL_TAC) >>
+ ‘is_v_bit' e’ by metis_tac[transform_e_is_v_bit] >> gs[] >>
+ ‘is_v_bit' e0’ by metis_tac[transform_e_is_v_bit] >> gs[] >>
+ ‘is_v_bit' e1’ by metis_tac[transform_e_is_v_bit] >> gs[] >>
+ (* First, get result of operation on cake_sem in proof goal *)
+ Cases_on ‘e’ >> (gs[is_v_bit'_def]) >>
+ Cases_on ‘e0’ >> (gs[is_v_bit'_def]) >>
+ Cases_on ‘e1’ >> (gs[is_v_bit'_def]) >>
+ Cases_on ‘v'’ >> (gs[is_v_bit'_def]) >>
+ Cases_on ‘v''’ >> (gs[is_v_bit'_def]) >>
+ Cases_on ‘v'''’ >> (gs[is_v_bit'_def]) >>
+ simp[e_exec_slice'_def, AllCaseEqs()] >>
+ (* Then, obtain everything involved
+  * in the operation from regular semantics by case analysis *)
+ Cases_on ‘e1''’ >> (gs[p4_exec_semTheory.is_v_bit_def]) >>
+ Cases_on ‘e2''’ >> (gs[p4_exec_semTheory.is_v_bit_def]) >>
+ Cases_on ‘e3’ >> (gs[p4_exec_semTheory.is_v_bit_def]) >>
+ Cases_on ‘v'’ >> (gs[p4_exec_semTheory.is_v_bit_def]) >>
+ Cases_on ‘v''’ >> (gs[p4_exec_semTheory.is_v_bit_def]) >>
+ Cases_on ‘v'''’ >> (gs[p4_exec_semTheory.is_v_bit_def]) >>
+ (* Apply regular operation *)
+ gvs[p4_exec_semTheory.e_exec_slice_def] >>
+ (* Connect the concrete values via translation *)
+ gvs[transform_e_def, transform_v_def] >>
+ (* Slice operation requires some extra stuff *)
+ Cases_on ‘p’ >>
+ Cases_on ‘p'’ >>
+ Cases_on ‘p''’ >>
+ gs[slice'_def, slice_def] >>
+ (* TODO: Slice operation in cake_sem also requires
+  * v2n q'' <= v2n q' /\ v2n q' < r /\ LENGTH q = r, which is a problem since the
+  * regular version just lets things be undefined... *)
+ cheat
+) >>
+(* Case 2b: e2' is not value *)
+‘is_v_bit' e0’ by metis_tac[transform_e_is_v_bit] >> gs[] >>
+‘is_v_bit' e1’ by metis_tac[transform_e_is_v_bit] >> gs[] >>
+‘~is_v_bit' e’ by metis_tac[transform_e_not_is_v_bit] >> gs[] >>
+(* 3. Rewrite transformation of final state *)
+qpat_x_assum ‘transform_e dict (e_slice e1' e2'' e3) = SOME e'2’ (fn thm => ASSUME_TAC $ ONCE_REWRITE_RULE [transform_e_def] thm >> gvs[app_opt_def, AllCaseEqs()]) >>
+(* 4. Use induction hypothesis *)
+metis_tac[]
+QED
+
+Theorem e_exec'_completeness:
+!e'1.
+e_exec'_complete e'1
+Proof
+‘(!e1. e_exec'_complete e1) /\ (!l. w_e_l_exec'_complete l) /\ (!p. w_e_exec'_complete p) /\ (!l. l_complete l)’ suffices_by (
+ fs []
+) >>
+irule e'_induction >>
+rpt strip_tac >- (
+ gs[w_e_l_exec'_complete_def, l_complete_def]
+) >- (
+ gs[l_complete_def]
+) >- (
+ (* Slice *)
+ metis_tac[e_exec'_completeness_slice]
+) >- (
+ (* Concatenation *)
+ metis_tac[e_exec'_completeness_concat]
+) >- (
+ (* Binary operation *)
+ metis_tac[e_exec'_completeness_binop]
+) >- (
+ (* Special: l_complete, recursive case *)
+ gs[l_complete_equiv, l_complete_exec_def]
+) >- (
+ (* Field access *)
+ metis_tac[e_exec'_completeness_acc]
+) >- (
+ (* Special: w_e_exec'_complete *)
+ gs[w_e_exec'_complete_def]
+) >- (
+ (* Cast *)
+ metis_tac[e_exec'_completeness_cast]
+) >- (
+ (* Select *)
+ metis_tac[e_exec'_completeness_select]
+) >- (
+ (* Unary operation *)
+ metis_tac[e_exec'_completeness_unop]
+) >- (
+ (* List *)
+ gs[e_exec'_complete_def] >>
+ rpt strip_tac >>
+ qpat_x_assum ‘transform_e dict e1 = SOME (e'_list l)’ (fn thm => assume_tac $ ONCE_REWRITE_RULE [transform_e_def] thm >> gvs[listTheory.UNZIP_MAP, AllCaseEqs()]) >> (
+  gs[p4_exec_semTheory.e_exec_def]
+ )
+) >- (
+ (* Function call *)
+ metis_tac[e_exec'_completeness_call]
+) >- (
+ (* Struct *)
+ metis_tac[e_exec'_completeness_struct]
+) >- (
+ (* Header *)
+ gs[e_exec'_complete_def] >>
+ rpt strip_tac >>
+ qpat_x_assum ‘transform_e dict e1 = SOME (e'_header b l)’ (fn thm => assume_tac $ ONCE_REWRITE_RULE [transform_e_def] thm >> gvs[listTheory.UNZIP_MAP, AllCaseEqs()]) >> (
+  gs[p4_exec_semTheory.e_exec_def]
+ )
+) >- (
+ (* w_e list: inductive case *)
+ Cases_on ‘p’ >>
+ gs[w_e_l_exec'_complete_def, l_complete_def, w_e_exec'_complete_def] >>
+ rpt strip_tac >>
+ Cases_on ‘i’ >> (
+  gs[listTheory.oEL_def]
+ ) >>
+ subgoal ‘MEM e (MAP SND l)’ >- (
+  gs[listTheory.oEL_EQ_EL, rich_listTheory.EL_MEM]
+ ) >>
+ metis_tac[l_complete_MEM]
+) >- (
+ (* Constant *)
+ gs[e_exec'_complete_def] >>
+ rpt strip_tac >>
+ qpat_x_assum ‘transform_e dict e1 = SOME (e'_v v)’ (fn thm => assume_tac $ ONCE_REWRITE_RULE [transform_e_def] thm >> gvs[listTheory.UNZIP_MAP, AllCaseEqs()]) >>
+ gs[p4_exec_semTheory.e_exec_def]
+) >>
+metis_tac[e_exec'_completeness_var]
+QED
+
+(**************)
+(* STMT-LEVEL *)
+(**************)
+
+(* TODO: Move *)
+(* TODO: Generalise from V1Model *)
+Definition transform_ctx_def:
+ transform_ctx dict ((apply_table_f, ext_map, func_map, b_func_map, pars_map, tbl_map):v1model_ascope ctx) =
+  transform_ext_map dict ext_map >>=
+  \ext_map'. transform_func_map dict func_map >>=
+  \func_map'. transform_func_map dict b_func_map >>=
+  \b_func_map'. transform_pars_map dict pars_map >>=
+  \pars_map'. transform_tbl_map dict tbl_map >>=
+  \tbl_map'. SOME (v1model_apply_table_f'', ext_map':v1model_ascope' ext_map', func_map':func_map', b_func_map':b_func_map', pars_map', tbl_map')
+End
+
+(* TODO: Move *)
+Definition transform_state_def:
+ transform_state dict ((ascope, g_scope_list, frame_list, status):v1model_ascope state) ctrl' =
+  transform_ascope dict ascope ctrl' >>=
+  \ascope'. transform_scope_list dict g_scope_list >>=
+  \g_scope_list'. transform_frame_list dict frame_list >>=
+  \frame_list'. transform_status dict status >>=
+  \status'. SOME ((ascope', g_scope_list', frame_list', status'):v1model_ascope' state')
+End
+
+(* TODO: Move *)
+Definition transform_stmt_list_def:
+ transform_stmt_list dict stmt_list =
+ oFOLDR (transform_stmt dict) stmt_list
+End
+
+(* TODO: Fix ctrl transformation *)
+Definition stmt_exec'_complete_def:
+ stmt_exec'_complete stmt'1 ctrl' =
+  !dict ctx ctx' ascope1 ascope'1 g_scope_list1 g_scope_list'1 funn1 funn'1 stmt1 stmt_stack1 stmt_stack'1 scope_list1 scope_list'1 status1 status'1 ctrl.
+  dict_bij dict ==>
+  transform_ctx dict ctx = SOME ctx' ==>
+  transform_ascope dict ascope1 ctrl = SOME ascope'1 ==>
+  transform_scope_list dict g_scope_list1 = SOME g_scope_list'1 ==>
+  transform_funn dict funn1 = SOME funn'1 ==>
+  transform_stmt dict stmt1 = SOME stmt'1 ==>
+  transform_stmt_list dict stmt_stack1 = SOME stmt_stack'1 ==>
+  transform_scope_list dict scope_list1 = SOME scope_list'1 ==>
+  transform_status dict status1 = SOME status'1 ==>
+  ?ctrl'.
+  !state2 state'2.
+  stmt_exec uninit_zero (ctx:v1model_ascope ctx) (ascope1, g_scope_list1:g_scope_list, [(funn1, stmt1::stmt_stack1, scope_list1)], status1) = SOME state2 ==>
+  transform_state dict state2 ctrl' = SOME state'2 ==>
+  stmt_exec' (ctx':v1model_ascope' ctx') (ascope'1, g_scope_list'1:g_scope_list', [(funn'1, stmt'1::stmt_stack'1, scope_list'1)], status'1) = SOME state'2
+End
+
+val stmt_exec'_completeness_tac =
+ simp[stmt_exec'_complete_def] >>
+ rpt strip_tac >>
+ (* The ctrl used in transform_ascope *)
+ qexists_tac ‘ctrl’ >>
+ rpt strip_tac >>
+ qpat_x_assum ‘transform_stmt dict stmt1 = SOME _’ (fn thm => assume_tac $ ONCE_REWRITE_RULE [transform_stmt_def] thm >> gvs[AllCaseEqs()]) >>
+ (* 2. Rewrite execution *)
+ PairCases_on ‘ctx’ >>
+ rename1 ‘(apply_table_f, ext_map, func_map, b_func_map, pars_map, tbl_map)’ >>
+ Cases_on ‘status1’ >> (
+  gvs[p4_exec_semTheory.stmt_exec_def, AllCaseEqs()]
+ ) >>
+ gvs[transform_status_def] >>
+ Cases_on ‘scope_list1’ >> (
+  gvs[p4_exec_semTheory.stmt_exec_def, AllCaseEqs()]
+ ) >>
+ gvs[transform_scope_list_def, oFOLDR_def] >>
+ Cases_on ‘state2’ >>
+ PairCases_on ‘r’ >>
+ rename1 ‘transform_state dict (ascope2,g_scope_list2,frame_list2,status2) ctrl = SOME state'2’
+;
+
+(* Simplifies the below theorem *)
+Definition transform_v_init_v_from_tau_def:
+transform_v_init_v_from_tau tau =
+ !tau' v' dict.
+ transform_v dict (arb_from_tau_gen uninit_zero tau) = SOME v' ==>
+ transform_tau dict tau = SOME tau' ==>
+ init_v_from_tau_cake tau' = v'
+End
+
+
+Theorem transform_v_struct_SOME:
+!s_l v_l w_v'_l dict.
+transform_v dict (v_struct $ ZIP(s_l, v_l)) = SOME (v'_struct w_v'_l) ==>
+?w_l. oFOLDR (ALOOKUP dict) s_l = SOME w_l /\
+?v'_l. oFOLDR (transform_v dict) v_l = SOME v'_l /\
+w_v'_l = ZIP(w_l, v'_l) /\
+LENGTH w_l = LENGTH s_l /\ LENGTH v'_l = LENGTH v_l
+Proof
+cheat
+QED
+
+Theorem transform_tau_xtl_SOME:
+!s_l tau_l w_tau'_l sty dict.
+transform_tau dict (tau_xtl sty (ZIP (s_l,tau_l))) = SOME (tau'_xtl sty w_tau'_l) ==>
+?w_l. oFOLDR (ALOOKUP dict) s_l = SOME w_l /\
+?tau'_l. oFOLDR (transform_tau dict) tau_l = SOME tau'_l /\
+w_tau'_l = ZIP(w_l, tau'_l) /\
+LENGTH w_l = LENGTH s_l /\ LENGTH tau'_l = LENGTH tau_l
+Proof
+cheat
+QED
+
+(* TODO: Move *)
+Definition OPTION_diamond_def:
+OPTION_diamond lf1 lf2 rf1 rf2 l =
+ !e1 e2.
+ MEM e1 l ==>
+ lf2 $ lf1 e1 = SOME e2 ==>
+ OPTION_BIND (rf1 e1) (SOME o rf2) = SOME e2
+End
+
+(* TODO: Move *)
+Theorem OPTION_diamond_oFOLDR_MAP:
+!l1 lf1 lf2 ll rf1 rl2 rf2.
+OPTION_diamond lf1 lf2 rf1 rf2 l1 ==>
+oFOLDR lf2 (MAP lf1 l1) = SOME ll ==>
+oFOLDR rf1 l1 = SOME rl2 ==>
+MAP rf2 rl2 = ll
+Proof
+Induct_on ‘l1’ >- (
+ gvs[oFOLDR_def, listTheory.MAP, OPTION_diamond_def]
+) >>  
+rpt strip_tac >>
+gvs[oFOLDR_def, listTheory.MAP] >>
+CONJ_TAC >- (
+ gs[OPTION_diamond_def] >>
+ qpat_x_assum ‘!e1 e2.
+          e1 = h \/ MEM e1 l1 ==>
+          lf2 (lf1 e1) = SOME e2 ==>
+          ?x. rf1 e1 = SOME x /\ rf2 x = e2’
+  (fn thm => assume_tac $ Q.SPECL [‘h’, ‘res’] thm) >>
+ gs[]
+) >>
+‘OPTION_diamond lf1 lf2 rf1 rf2 l1’ by (
+ gs[OPTION_diamond_def]
+) >>
+metis_tac[]
+QED
+
+Theorem transform_tau_oFOLDR:
+!tau_l tau'_l tau tau' dict.
+oFOLDR (transform_tau dict) tau_l = SOME tau'_l ==>
+MEM tau tau_l ==>
+?tau'. transform_tau dict tau = SOME tau'
+Proof
+Induct >> (
+ gvs[listTheory.MEM]
+) >>
+rpt strip_tac >> (
+ gs[oFOLDR_def]
+)
+QED
+
+Theorem transform_v_init_v_from_tau:
+!tau tau' v' dict.
+transform_v dict (arb_from_tau_gen uninit_zero tau) = SOME v' ==>
+transform_tau dict tau = SOME tau' ==>
+init_v_from_tau_cake tau' = v'
+Proof
+‘(!tau. transform_v_init_v_from_tau tau) /\
+ (!l:(string # tau) list. (\xtl. EVERY transform_v_init_v_from_tau $ MAP SND xtl) l) /\
+ !p:(string # tau). (\xt. transform_v_init_v_from_tau $ SND xt) p’ suffices_by (
+ metis_tac[transform_v_init_v_from_tau_def]
+) >>
+irule tau_induction >>
+gs[transform_v_init_v_from_tau_def] >>
+rpt strip_tac >- (
+ gvs[Once transform_tau_def, p4_exec_semTheory.arb_from_tau_gen_def] >>
+ gvs[p4_exec_semTheory.uninit_bit_def, p4_exec_semTheory.uninit_num_def, transform_v_def, init_v_from_tau_cake_def]
+) >- (
+ gvs[Once transform_tau_def, p4_exec_semTheory.arb_from_tau_gen_def] >>
+ gvs[p4_exec_semTheory.uninit_bit_def, p4_exec_semTheory.uninit_num_def, transform_v_def, init_v_from_tau_cake_def]
+) >- (
+ gvs[Once transform_tau_def, p4_exec_semTheory.arb_from_tau_gen_def] >>
+ gvs[p4_exec_semTheory.uninit_bit_def, p4_exec_semTheory.uninit_num_def, transform_v_def, init_v_from_tau_cake_def]
+) >- (
+ Cases_on ‘s’ >> (
+   gvs[Once transform_v_def, Once transform_tau_def, p4_exec_semTheory.arb_from_tau_gen_def, 
+       init_v_from_tau_cake_def, AllCaseEqs()] >- (
+    gs[transform_tau_def, init_v_from_tau_cake_def, p4_exec_semTheory.uninit_bit_def]
+   )
+ ) >- (
+  (* TODO: Get this in a better way to unify cases *)
+  ‘struct_ty' = struct_ty_struct’ by cheat >> gvs[] >>
+   gvs[init_v_from_tau_cake_def] >>
+  CONJ_TAC >- (
+   qpat_x_assum ‘transform_v_init_v_from_tau tau''’ (fn thm => assume_tac $ REWRITE_RULE [transform_v_init_v_from_tau_def] thm) >>
+   metis_tac[]
+  ) >>
+  (* TODO: The interesting part... *)
+  ‘?s_l tau_l. t'' = ZIP(s_l, tau_l) /\ LENGTH s_l = LENGTH tau_l’ by cheat >> gvs[] >>
+  gvs[listTheory.MAP_ZIP] >>
+  (* Clarification of t': *)
+  ‘MAP (\(x,t). (x,arb_from_tau_gen uninit_zero t)) (ZIP (s_l,tau_l)) = ZIP (s_l, MAP (arb_from_tau_gen uninit_zero) tau_l)’ by cheat >> gvs[] >>
+  imp_res_tac transform_v_struct_SOME >>
+  gvs[] >>
+  imp_res_tac transform_tau_xtl_SOME >>
+  gvs[] >>
+  ‘MAP (\(x,t). (x,init_v_from_tau_cake t)) (ZIP (w_l,tau'_l)) = (ZIP (w_l, MAP init_v_from_tau_cake tau'_l))’ by cheat >> gvs[] >>
+  ‘MAP init_v_from_tau_cake tau'_l = v'_l’ suffices_by gs[] >>
+  irule $ ISPECL [“tau_l:tau list”, “arb_from_tau_gen uninit_zero”] OPTION_diamond_oFOLDR_MAP >>
+  qexistsl_tac[‘transform_v dict’, ‘transform_tau dict’, ‘tau_l’] >>
+  gs[OPTION_diamond_def] >>
+  rpt strip_tac >>
+  gs[listTheory.EVERY_MEM] >>
+  res_tac >>
+  gs[transform_v_init_v_from_tau_def] >>
+  ‘?tau1. transform_tau dict e1 = SOME tau1’ by metis_tac[transform_tau_oFOLDR] >>
+  metis_tac[]
+ ) >>
+ (* Header: *)
+ ‘struct_ty' = struct_ty_header’ by cheat >> gvs[] >>
+  gvs[init_v_from_tau_cake_def, p4_exec_semTheory.uninit_bit_def] >>
+ CONJ_TAC >- (
+  qpat_x_assum ‘transform_v_init_v_from_tau tau''’ (fn thm => assume_tac $ REWRITE_RULE [transform_v_init_v_from_tau_def] thm) >>
+  metis_tac[]
+ ) >>
+ ‘?s_l tau_l. t'' = ZIP(s_l, tau_l) /\ LENGTH s_l = LENGTH tau_l’ by cheat >> gvs[] >>
+ gvs[listTheory.MAP_ZIP] >>
+ (* Clarification of t': *)
+ ‘MAP (\(x,t). (x,arb_from_tau_gen uninit_zero t)) (ZIP (s_l,tau_l)) = ZIP (s_l, MAP (arb_from_tau_gen uninit_zero) tau_l)’ by cheat >> gvs[] >>
+ imp_res_tac transform_v_struct_SOME >>
+ gvs[] >>
+ imp_res_tac transform_tau_xtl_SOME >>
+ gvs[] >>
+ ‘MAP (\(x,t). (x,init_v_from_tau_cake t)) (ZIP (w_l,tau'_l)) = (ZIP (w_l, MAP init_v_from_tau_cake tau'_l))’ by cheat >> gvs[] >>
+ ‘MAP init_v_from_tau_cake tau'_l = v'_l’ suffices_by gs[] >>
+ irule $ ISPECL [“tau_l:tau list”, “arb_from_tau_gen uninit_zero”] OPTION_diamond_oFOLDR_MAP >>
+ qexistsl_tac[‘transform_v dict’, ‘transform_tau dict’, ‘tau_l’] >>
+ gs[OPTION_diamond_def] >>
+ rpt strip_tac >>
+ gs[listTheory.EVERY_MEM] >>
+ res_tac >>
+ gs[transform_v_init_v_from_tau_def] >>
+ ‘?tau1. transform_tau dict e1 = SOME tau1’ by metis_tac[transform_tau_oFOLDR] >>
+ metis_tac[]
+) >>
+gvs[transform_tau_def, p4_exec_semTheory.arb_from_tau_gen_def] >>
+gvs[p4_exec_semTheory.uninit_bit_def, p4_exec_semTheory.uninit_num_def, transform_v_def, init_v_from_tau_cake_def] >>
+gs[rich_listTheory.REPLICATE_GENLIST] >>
+irule listTheory.GENLIST_CONG >>
+simp[combinTheory.K_THM]
+QED
+
+Theorem transform_t_scope_list_declare_fresh_scope_equiv:
+!t_scope t_scope' scope' dict.
+transform_scope dict (declare_list_in_fresh_scope_exec uninit_zero t_scope) = SOME scope' ==>
+transform_t_scope_list dict t_scope = SOME t_scope' ==>
+declare_list_in_fresh_scope' t_scope' = scope'
+Proof
+Induct >- (
+rpt strip_tac >>
+gvs[p4_exec_semTheory.declare_list_in_fresh_scope_exec_def, declare_list_in_fresh_scope'_def,
+   transform_scope_def, transform_t_scope_list_def, oFOLDR_def]
+) >>
+rpt strip_tac >>
+PairCases_on ‘h’ >>
+rename1 ‘(varn, tau, lval_opt)’ >>
+gvs[p4_exec_semTheory.declare_list_in_fresh_scope_exec_def, declare_list_in_fresh_scope'_def,
+   transform_scope_def, transform_t_scope_list_def, oFOLDR_def] >>
+CONJ_TAC >- (
+ PairCases_on ‘res'’ >>
+ gs[] >>
+ PairCases_on ‘res’ >>
+ gvs[transform_scope_entry_def, transform_t_scope_def, AllCaseEqs()] >>
+ metis_tac[transform_v_init_v_from_tau]
+) >>
+qpat_x_assum ‘!t_scope''. _’ (fn thm => irule thm) >>
+metis_tac[]
+QED
+
+Theorem stmt_exec'_completeness:
+!ctrl' stmt'1.
+stmt_exec'_complete stmt'1 ctrl'
+Proof
+assume_tac e_exec'_completeness >>
+strip_tac >>
+‘!stmt'1. (\stmt'. !ctrl'. stmt_exec'_complete stmt' ctrl') stmt'1’ suffices_by (
+ fs[]
+) >>
+irule stmt'_induction >> (
+ gs[]
+) >>
+rpt strip_tac >- (
+ (*********)
+ (* Empty *)
+ gs[stmt_exec'_complete_def] >>
+ rpt strip_tac >>
+ (* The ctrl used in transform_ascope *)
+ qexists_tac ‘ctrl’ >>
+ rpt strip_tac >>
+ qpat_x_assum ‘transform_stmt dict stmt1 = SOME _’ (fn thm => assume_tac $ ONCE_REWRITE_RULE [transform_stmt_def] thm >> gvs[AllCaseEqs()]) >>
+ (* 2. Rewrite execution *)
+ PairCases_on ‘ctx’ >>
+ rename1 ‘(apply_table_f, ext_map, func_map, b_func_map, pars_map, tbl_map)’ >>
+ Cases_on ‘status1’ >> Cases_on ‘scope_list1’ >> Cases_on ‘stmt_stack1’ >> (
+  gvs[p4_exec_semTheory.stmt_exec_def, AllCaseEqs()]
+ ) >>
+ (* 3. Finish transformations with the results *)
+ gvs[transform_status_def, transform_stmt_list_def, transform_scope_list_def, transform_state_def, transform_frame_list_def, transform_frame_def, oFOLDR_def, AllCaseEqs()] >>
+ (* 4. Rewrite the cake_sem execution *)
+ gvs[stmt_exec'_def, AllCaseEqs()]
+) >- (
+ (**********)
+ (* Extern *)
+ (* TODO: This has to go through all the cases of the extern functions... *)
+ gs[stmt_exec'_complete_def] >>
+ rpt strip_tac >>
+ (* The ctrl used in transform_ascope *)
+ qexists_tac ‘ctrl’ >>
+ rpt strip_tac >>
+ qpat_x_assum ‘transform_stmt dict stmt1 = SOME _’ (fn thm => assume_tac $ ONCE_REWRITE_RULE [transform_stmt_def] thm >> gvs[AllCaseEqs()]) >>
+ (* 2. Rewrite execution *)
+ PairCases_on ‘ctx’ >>
+ rename1 ‘(apply_table_f, ext_map, func_map, b_func_map, pars_map, tbl_map)’ >>
+ Cases_on ‘status1’ >> Cases_on ‘scope_list1’ >> Cases_on ‘stmt_stack1’ >> (
+  gvs[p4_exec_semTheory.stmt_exec_def, AllCaseEqs()]
+ ) >- (
+  (* Case 1: At bottom of stmt_stack *)
+  (* 3. Finish transformations with the results *)
+  gvs[transform_status_def, transform_stmt_list_def, transform_scope_list_def, transform_state_def, transform_frame_list_def, transform_frame_def, oFOLDR_def, AllCaseEqs()] >> (
+   (* 4. Rewrite the cake_sem execution *)
+   PairCases_on ‘ctx'’ >>
+   rename1 ‘(apply_table_f', ext_map', func_map', b_func_map', pars_map', tbl_map')’ >>
+   gvs[stmt_exec'_def, AllCaseEqs()] >>
+   cheat
+  )
+ ) >>
+ (* Case 2: Some stmt_stack below *)
+ (* 3. Finish transformations with the results *)
+ gvs[transform_status_def, transform_stmt_list_def, transform_scope_list_def, transform_state_def, transform_frame_list_def, transform_frame_def, oFOLDR_def, AllCaseEqs()] >> (
+  (* 4. Rewrite the cake_sem execution *)
+  PairCases_on ‘ctx'’ >>
+  rename1 ‘(apply_table_f', ext_map', func_map', b_func_map', pars_map', tbl_map')’ >>
+  gvs[stmt_exec'_def, AllCaseEqs()] >>
+  cheat
+ )
+) >- (
+ (*********************)
+ (* Table application *)
+ gs[stmt_exec'_complete_def] >>
+ rpt strip_tac >>
+ (* The ctrl used in transform_ascope *)
+ qexists_tac ‘ctrl’ >>
+ rpt strip_tac >>
+ qpat_x_assum ‘transform_stmt dict stmt1 = SOME _’ (fn thm => assume_tac $ ONCE_REWRITE_RULE [transform_stmt_def] thm >> gvs[AllCaseEqs()]) >>
+ (* 2. Rewrite execution *)
+ PairCases_on ‘ctx’ >>
+ rename1 ‘(apply_table_f, ext_map, func_map, b_func_map, pars_map, tbl_map)’ >>
+ Cases_on ‘status1’ >> Cases_on ‘scope_list1’ >> Cases_on ‘stmt_stack1’ >> (
+  gvs[p4_exec_semTheory.stmt_exec_def, AllCaseEqs()]
+ ) >>
+ cheat
+(*
+ (* 3. Finish transformations with the results *)
+ gvs[transform_status_def, transform_stmt_list_def, transform_scope_list_def, transform_state_def, transform_frame_list_def, transform_frame_def, oFOLDR_def, AllCaseEqs()] >>
+ (* 4. Rewrite the cake_sem execution *)
+ PairCases_on ‘ctx'’ >>
+ rename1 ‘(apply_table_f', ext_map', func_map', b_func_map', pars_map', tbl_map')’ >>
+ gvs[stmt_exec'_def, AllCaseEqs()] >>
+ (* Preservation of all the properties... *)
+ cheat
+*)
+) >- (
+ (**********)
+ (* Return *)
+ gs[stmt_exec'_complete_def] >>
+ rpt strip_tac >>
+ (* The ctrl used in transform_ascope *)
+ qexists_tac ‘ctrl’ >>
+ rpt strip_tac >>
+ qpat_x_assum ‘transform_stmt dict stmt1 = SOME _’ (fn thm => assume_tac $ ONCE_REWRITE_RULE [transform_stmt_def] thm >> gvs[AllCaseEqs()]) >>
+ (* 2. Rewrite execution *)
+ PairCases_on ‘ctx’ >>
+ rename1 ‘(apply_table_f, ext_map, func_map, b_func_map, pars_map, tbl_map)’ >>
+ Cases_on ‘status1’ >> Cases_on ‘scope_list1’ >> Cases_on ‘stmt_stack1’ >> (
+  gvs[p4_exec_semTheory.stmt_exec_def, AllCaseEqs()]
+ ) >> (
+  cheat
+  (*
+  (* 5 different combinations possible *)
+  (* 3. Finish transformations with the results *)
+  gvs[transform_status_def, transform_stmt_list_def, transform_scope_list_def, transform_state_def, transform_frame_list_def, transform_frame_def, oFOLDR_def, AllCaseEqs()] >>
+  (* 4. Rewrite the cake_sem execution *)
+  PairCases_on ‘ctx'’ >>
+  rename1 ‘(apply_table_f', ext_map', func_map', b_func_map', pars_map', tbl_map')’ >>
+  gvs[stmt_exec'_def, AllCaseEqs()] >>
+  (* Preservation of all the properties... *)
+  cheat
+*)
+ )
+) >- (
+ (*********)
+ (* Trans *)
+ gs[stmt_exec'_complete_def] >>
+ rpt strip_tac >>
+ (* The ctrl used in transform_ascope *)
+ qexists_tac ‘ctrl’ >>
+ rpt strip_tac >>
+ qpat_x_assum ‘transform_stmt dict stmt1 = SOME _’ (fn thm => assume_tac $ ONCE_REWRITE_RULE [transform_stmt_def] thm >> gvs[AllCaseEqs()]) >>
+ (* 2. Rewrite execution *)
+ PairCases_on ‘ctx’ >>
+ rename1 ‘(apply_table_f, ext_map, func_map, b_func_map, pars_map, tbl_map)’ >>
+ Cases_on ‘status1’ >> Cases_on ‘scope_list1’ >> Cases_on ‘stmt_stack1’ >> (
+  gvs[p4_exec_semTheory.stmt_exec_def, AllCaseEqs()]
+ ) >> (
+  cheat
+(*
+  (* 5 different combinations possible *)
+  (* 3. Finish transformations with the results *)
+  gvs[transform_status_def, transform_stmt_list_def, transform_scope_list_def, transform_state_def, transform_frame_list_def, transform_frame_def, oFOLDR_def, AllCaseEqs()] >>
+  (* 4. Rewrite the cake_sem execution *)
+  PairCases_on ‘ctx'’ >>
+  rename1 ‘(apply_table_f', ext_map', func_map', b_func_map', pars_map', tbl_map')’ >>
+  gvs[stmt_exec'_def, AllCaseEqs()] >>
+  (* Preservation of all the properties... *)
+  cheat
+*)
+ )
+) >- (
+ (**************)
+ (* Assignment *)
+ gs[stmt_exec'_complete_def] >>
+ rpt strip_tac >>
+ (* The ctrl used in transform_ascope *)
+ qexists_tac ‘ctrl’ >>
+ rpt strip_tac >>
+ qpat_x_assum ‘transform_stmt dict stmt1 = SOME _’ (fn thm => assume_tac $ ONCE_REWRITE_RULE [transform_stmt_def] thm >> gvs[AllCaseEqs()]) >>
+ (* 2. Rewrite execution *)
+ PairCases_on ‘ctx’ >>
+ rename1 ‘(apply_table_f, ext_map, func_map, b_func_map, pars_map, tbl_map)’ >>
+ Cases_on ‘status1’ >> Cases_on ‘scope_list1’ >> Cases_on ‘stmt_stack1’ >> (
+  gvs[p4_exec_semTheory.stmt_exec_def, AllCaseEqs()]
+ ) >> (
+  cheat
+(*
+  (* 5 different combinations possible *)
+  (* 3. Finish transformations with the results *)
+  gvs[transform_status_def, transform_stmt_list_def, transform_scope_list_def, transform_state_def, transform_frame_list_def, transform_frame_def, oFOLDR_def, AllCaseEqs()] >>
+  (* 4. Rewrite the cake_sem execution *)
+  PairCases_on ‘ctx'’ >>
+  rename1 ‘(apply_table_f', ext_map', func_map', b_func_map', pars_map', tbl_map')’ >>
+  gvs[stmt_exec'_def, AllCaseEqs()] >>
+  (* Preservation of all the properties... *)
+  cheat
+*)
+ )
+) >- (
+ (************)
+ (* Sequence *)
+ simp[stmt_exec'_complete_def] >>
+ rpt strip_tac >>
+ (* The ctrl used in transform_ascope *)
+ qexists_tac ‘ctrl’ >>
+ rpt strip_tac >>
+ qpat_x_assum ‘transform_stmt dict stmt1 = SOME _’ (fn thm => assume_tac $ ONCE_REWRITE_RULE [transform_stmt_def] thm >> gvs[AllCaseEqs()]) >>
+ (* 2. Rewrite execution *)
+ PairCases_on ‘ctx’ >>
+ rename1 ‘(apply_table_f, ext_map, func_map, b_func_map, pars_map, tbl_map)’ >>
+ Cases_on ‘status1’ >> (
+  gvs[p4_exec_semTheory.stmt_exec_def, AllCaseEqs()]
+ ) >>
+ gvs[transform_status_def] >>
+ Cases_on ‘scope_list1’ >> (
+  gvs[p4_exec_semTheory.stmt_exec_def, AllCaseEqs()]
+ ) >>
+ gvs[transform_scope_list_def, oFOLDR_def] >>
+ Cases_on ‘state2’ >>
+ PairCases_on ‘r’ >>
+ rename1 ‘transform_state dict (ascope2,g_scope_list2,frame_list2,status2) ctrl = SOME state'2’ >>
+ gs[p4_exec_semTheory.exec_stmt_seq_SOME_REWRS] >>
+ Cases_on ‘is_empty stmt1'’ >> (
+  gvs[]
+ ) >> (
+  (* 4 different combinations possible *)
+  (* 3. Finish transformations with the results *)
+  gvs[transform_status_def, transform_stmt_list_def, transform_scope_list_def, transform_state_def, transform_frame_list_def, transform_frame_def, oFOLDR_def, AllCaseEqs()] >>
+  (* 4. Rewrite the cake_sem execution *)
+  PairCases_on ‘ctx'’ >>
+  rename1 ‘(apply_table_f', ext_map', func_map', b_func_map', pars_map', tbl_map')’ >>
+  gvs[stmt_exec'_def, AllCaseEqs()] >>
+  (* Apply induction hypothesis depending on whether you end up with stmt_exec in assums *)
+  cheat
+ )
+) >- (
+ (***************)
+ (* Conditional *)
+ (* Shared incipit tactic: *)
+ simp[stmt_exec'_complete_def] >>
+ rpt strip_tac >>
+ (* The ctrl used in transform_ascope *)
+ qexists_tac ‘ctrl’ >>
+ rpt strip_tac >>
+ qpat_x_assum ‘transform_stmt dict stmt1 = SOME _’ (fn thm => assume_tac $ ONCE_REWRITE_RULE [transform_stmt_def] thm >> gvs[AllCaseEqs()]) >>
+ (* 2. Rewrite execution *)
+ PairCases_on ‘ctx’ >>
+ rename1 ‘(apply_table_f, ext_map, func_map, b_func_map, pars_map, tbl_map)’ >>
+ Cases_on ‘status1’ >> (
+  gvs[p4_exec_semTheory.stmt_exec_def, AllCaseEqs()]
+ ) >>
+ gvs[transform_status_def] >>
+ Cases_on ‘scope_list1’ >> (
+  gvs[p4_exec_semTheory.stmt_exec_def, AllCaseEqs()]
+ ) >>
+ gvs[transform_scope_list_def, oFOLDR_def] >>
+ Cases_on ‘state2’ >>
+ PairCases_on ‘r’ >>
+ rename1 ‘transform_state dict (ascope2,g_scope_list2,frame_list2,status2) ctrl = SOME state'2’ >>
+ (* End of shared incipit *)
+
+ gs[p4_exec_semTheory.exec_stmt_cond_SOME_REWRS] >>
+ Cases_on ‘is_v_bool e'’ >> (
+  gs[]
+ ) >- (
+  (* Case condition is reduced *)
+  Cases_on ‘b’ >> (
+   gs[]
+  ) >- (
+   (* Case condition holds *)
+   cheat
+  ) >>
+  (* Case condition doesn't hold *)
+  cheat
+ ) >>
+ (* Case condition is not reduced: use expression completeness *)
+ cheat
+) >>
+(*********)
+(* Block *)
+(* 1. Common incipit tactic *)
+stmt_exec'_completeness_tac >>
+(* 2. Use rewriting theorem *)
+gvs[p4_exec_semTheory.exec_stmt_block_SOME_REWRS] >>
+(* 3. Perform transformations *)
+gvs[transform_state_def, transform_frame_list_def, transform_frame_def, transform_status_def, transform_scope_list_def, oFOLDR_def, AllCaseEqs()] >>
+qpat_x_assum ‘transform_stmt dict stmt_empty = SOME _’ (fn thm => assume_tac $ ONCE_REWRITE_RULE [transform_stmt_def] thm >> gvs[AllCaseEqs()]) >>
+
+(* 4. Now try to rewrite the stmt_exec' in the goal *)
+PairCases_on ‘ctx'’ >>
+rename1 ‘(apply_table_f', ext_map', func_map', b_func_map', pars_map', tbl_map')’ >>
+Cases_on ‘stmt_stack1’ >> (
+ gvs[transform_stmt_list_def, oFOLDR_def, AllCaseEqs()]
+) >> (
+ (* Same lemma needed for both cases *)
+ gvs[stmt_exec'_def, AllCaseEqs()] >>
+ metis_tac[transform_t_scope_list_declare_fresh_scope_equiv]
+)
+QED
+
+(***************)
+(* FRAME-LEVEL *)
+(***************)
+
+Definition frames_exec'_complete_def:
+ frames_exec'_complete frame_list'1 ctrl' =
+  !dict ctx ctx' ascope1 ascope'1 g_scope_list1 g_scope_list'1 frame_list1 status1 status'1 ctrl.
+  dict_bij dict ==>
+  transform_ctx dict ctx = SOME ctx' ==>
+  transform_ascope dict ascope1 ctrl = SOME ascope'1 ==>
+  transform_scope_list dict g_scope_list1 = SOME g_scope_list'1 ==>
+  transform_frame_list dict frame_list1 = SOME frame_list'1 ==>
+  transform_status dict status1 = SOME status'1 ==>
+  ?ctrl'.
+  !state2 state'2.
+  frames_exec uninit_zero (ctx:v1model_ascope ctx) (ascope1, g_scope_list1:g_scope_list, frame_list1, status1) = SOME state2 ==>
+  transform_state dict state2 ctrl' = SOME state'2 ==>
+  frames_exec' (ctx':v1model_ascope' ctx') (ascope'1, g_scope_list'1:g_scope_list', frame_list'1, status'1) = SOME state'2
+End
+
+Theorem frames_exec'_completeness:
+!ctrl' frame_list'1.
+frames_exec'_complete frame_list'1 ctrl'
+Proof
+cheat
+QED
+
+(*************)
+(* TOP-LEVEL *)
+(*************)
+
+Theorem arch_exec'_completeness:
+!dict ab_list pblock_map ffblock_map input_f output_f copyin_pbl copyout_pbl apply_table_f ext_map func_map ab_list' pblock_map' ffblock_map' input_f' output_f' copyin_pbl' copyout_pbl' apply_table_f' ext_map' func_map' ctrl s1 s2 s'1 s'2.
+dict_bij dict ==>
+transform_actx dict (ab_list,pblock_map,ffblock_map,input_f,output_f,copyin_pbl,
+                     copyout_pbl,apply_table_f,ext_map,func_map) = SOME (ab_list',pblock_map',ext_map',func_map') ==>
+(* TODO: Need to state and assume completeness of the following:
+ffblock_map'
+input_f'
+output_f'
+copyin_pbl'
+copyout_pbl'
+apply_table_f'
+*)
+transform_astate dict s1 ctrl = SOME s'1 ==>
+arch_exec uninit_zero (ab_list,pblock_map,ffblock_map,input_f,output_f,
+                 copyin_pbl,copyout_pbl,apply_table_f,ext_map,func_map) s1 = SOME s2 ==>
+transform_astate dict s2 ctrl = SOME s'2 ==>
+arch_exec' (ab_list',pblock_map',ffblock_map',input_f',output_f',
+                  copyin_pbl',copyout_pbl',apply_table_f',ext_map',func_map') s'1 = SOME s'2
+Proof
+rpt strip_tac >>
+cheat
+QED
+
+(* TODO: Copy-paste of p4_contract'_def from p4_symb_execScript.sml *)
+Definition p4_contract_def:
+ p4_contract P ctx Q <=>
+  !s.
+   P s ==>
+   ?n. arch_multi_exec ctx s n <> NONE /\
+       !s'. arch_multi_exec ctx s n = SOME s' ==> Q s'
+End
+
+Definition p4_contract'_def:
+ p4_contract' P ctx Q <=>
+  !s.
+   P s ==>
+   ?n. arch_multi_exec' ctx s n <> NONE /\
+       !s'. arch_multi_exec' ctx s n = SOME s' ==> Q s'
+End
+
+(* TODO: Translating total-correctness contract requires completeness... *)
+(* TODO: Formulate new version of arch_multi_exec using uninit_zero that can be used by
+ * symbolic execution *)
+Theorem arch_multi_exec'_completeness:
+!dict ab_list pblock_map ffblock_map input_f output_f copyin_pbl copyout_pbl apply_table_f ext_map func_map ab_list' pblock_map' ffblock_map' input_f' output_f' copyin_pbl' copyout_pbl' apply_table_f' ext_map' func_map' ctrl s1 s2 s'1 s'2 n.
+dict_bij dict ==>
+transform_actx dict (ab_list,pblock_map,ffblock_map,input_f,output_f,copyin_pbl,
+                     copyout_pbl,apply_table_f,ext_map,func_map) = SOME (ab_list',pblock_map',ext_map',func_map') ==>
+(* TODO: Need to state and assume completeness of the following:
+ffblock_map'
+input_f'
+output_f'
+copyin_pbl'
+copyout_pbl'
+apply_table_f'
+*)
+transform_astate dict s1 ctrl = SOME s'1 ==>
+arch_multi_exec (ab_list,pblock_map,ffblock_map,input_f,output_f,
+                 copyin_pbl,copyout_pbl,apply_table_f,ext_map,func_map) s1 n = SOME s2 ==>
+transform_astate dict s2 ctrl = SOME s'2 ==>
+arch_multi_exec' (ab_list',pblock_map',ffblock_map',input_f',output_f',
+                  copyin_pbl',copyout_pbl',apply_table_f',ext_map',func_map') s'1 n = SOME s'2
+Proof
+rpt strip_tac >>
+cheat
+QED
+
+Theorem cake_sem_contract:
+!dict ab_list pblock_map ffblock_map input_f output_f copyin_pbl copyout_pbl apply_table_f ext_map func_map ab_list' pblock_map' ffblock_map' input_f' output_f' copyin_pbl' copyout_pbl' apply_table_f' ext_map' func_map' ctrl P' P Q Q'.
+dict_bij dict ==>
+(* TODO: Need to state and assume completeness of the following:
+ffblock_map'
+input_f'
+output_f'
+copyin_pbl'
+copyout_pbl'
+apply_table_f'
+*)
+transform_actx dict (ab_list,pblock_map,ffblock_map,input_f,output_f,copyin_pbl,
+                     copyout_pbl,apply_table_f,ext_map,func_map) = SOME (ab_list',pblock_map',ext_map',func_map') ==>
+(* Note this has to be computed *)
+(!s s'. transform_astate dict s ctrl = SOME s' ==>
+     (P' s' ==> P s) /\ (Q s ==> Q' s')) ==>
+p4_contract P (ab_list,pblock_map,ffblock_map,input_f,output_f,copyin_pbl,
+               copyout_pbl,apply_table_f,ext_map,func_map) Q ==>
+               
+p4_contract' P' (ab_list',pblock_map',ffblock_map',input_f',output_f',copyin_pbl',copyout_pbl',apply_table_f',ext_map',func_map') Q'
+Proof
+gvs[p4_contract_def] >>
+rpt strip_tac >>
+gs[p4_contract'_def] >>
+rpt strip_tac >>
+rename1 ‘P' s'’ >>
+(* TODO: In order for this to be provable, the contracts need to also include a notion of
+ * "valid state" in both precondition and postcondition, which entails the astates can always be
+ * translated using some dictionary (computed from the individual program).
+ *
+ * valid_astate dict s
+ *
+ * Look into what the causes of NONE may be in transform_astate, if it's only dictionary lookup
+ * or something else. This has some similarity to the prerequisites of the BIR lifting *)
+(* TODO: Note that the current transform_astate definition would only allow to prove this for
+ * states with empty arch frame lists (arch_frame_list'_empty), but that's probably OK. *)
+‘?s. transform_astate dict s ctrl = SOME s'’ by cheat >>
+‘(P' s' ⇒ P s) ∧ (Q s ⇒ Q' s')’ by metis_tac[] >>
+‘P s’ by metis_tac[] >>
+‘?n. arch_multi_exec
+                  (ab_list,pblock_map,ffblock_map,input_f,output_f,
+                   copyin_pbl,copyout_pbl,apply_table_f,ext_map,func_map) s n ≠
+                NONE ∧
+                ∀s'.
+                  arch_multi_exec
+                    (ab_list,pblock_map,ffblock_map,input_f,output_f,
+                     copyin_pbl,copyout_pbl,apply_table_f,ext_map,func_map) s
+                    n =
+                  SOME s' ⇒
+                  Q s'’ by metis_tac[] >>
+‘?s2. arch_multi_exec
+            (ab_list,pblock_map,ffblock_map,input_f,output_f,copyin_pbl,
+             copyout_pbl,apply_table_f,ext_map,func_map) s n = SOME s2’ by (
+ Cases_on ‘arch_multi_exec
+           (ab_list,pblock_map,ffblock_map,input_f,output_f,copyin_pbl,
+            copyout_pbl,apply_table_f,ext_map,func_map) s n’ >> (gs[])
+) >>
+‘Q s2’ by metis_tac[] >>
+qexists_tac ‘n’ >>
+gs[] >>
+(* TODO: By "valid_state" *)
+‘?s'2. transform_astate dict s2 ctrl = SOME s'2’ by cheat >>
+‘!output_f' input_f' ffblock_map' copyout_pbl' copyin_pbl'
+     apply_table_f'.
+   arch_multi_exec'
+     (ab_list',pblock_map',ffblock_map',input_f',output_f',
+      copyin_pbl',copyout_pbl',apply_table_f',ext_map',func_map') s' n =
+   SOME s'2’ by metis_tac[arch_multi_exec'_completeness] >>
+gvs[] >>
+metis_tac[]
+QED
+
+val _ = export_theory ();
